sha/verif_hmacADT_init_part1.v
@@ -8,53 +8,187 @@ Require Import sha.spec_sha.
 Require Import sha.sha_lemmas.
 Require Import sha.HMAC_functional_prog.
 
-Require Import sha.hmac091c.
+Require Import sha.hmac_NK.
 Require Import sha.HMAC_lemmas.
-Require Import sha.spec_hmac.
+Require Import sha.spec_hmacADT.
 
-Definition initPostKeyNullConditional r (c:val) (k: val) h key : mpred:=
+Definition initPostKeyNullConditional l r (c:val) (k: val) h key ctxkey: mpred:=
   match k with
     Vint z => if Int.eq z Int.zero
-              then if zeq r Z0 then hmacstate_PreInitNull key h c else FF
+              then if zeq r Z0 
+                   then (hmacstate_PreInitNull key h c) * (data_at_ Tsh (tarray tuchar 64) ctxkey)
+                   else FF
+              else FF
+  | Vptr b ofs => if zeq r 0 then FF 
+                  else EX ll:_,
+                      !!(Forall isbyteZ key /\ has_lengthK ll key /\ l = Vint(Int.repr ll)) &&
+                    ((data_at Tsh t_struct_hmac_ctx_st keyedHMS c) *
+                     (data_at Tsh (tarray tuchar 64) (map Vint (map Int.repr (HMAC_SHA256.mkKey key)))
+                      ctxkey) *
+                    (array_at tuchar Tsh (tuchars (map Int.repr key)) 0 (Zlength key)
+                      (Vptr b ofs)))
+  | _ => FF
+  end. (*
+Definition initPostKeyNullConditional r (c:val) (k: val) h key ctxkey: mpred:=
+  match k with
+    Vint z => if Int.eq z Int.zero
+              then if zeq r Z0 
+                   then (hmacstate_PreInitNull key h c) * (data_at_ Tsh (tarray tuchar 64) ctxkey)
+                   else FF
               else FF
   | Vptr b ofs => if zeq r 0 then FF 
                   else !!(Forall isbyteZ key) &&
-                    ((data_at Tsh t_struct_hmac_ctx_st (keyedHMS key) c) *
+                    ((data_at Tsh t_struct_hmac_ctx_st keyedHMS c) *
+                     (data_at Tsh (tarray tuchar 64) (map Vint (map Int.repr (HMAC_SHA256.mkKey key)))
+                      ctxkey) *
                     (array_at tuchar Tsh (tuchars (map Int.repr key)) 0 (Zlength key)
                       (Vptr b ofs)))
   | _ => FF
   end.
-
+*)
 Lemma hmac_init_part1: forall
 (Espec : OracleKind)
 (c : val)
 (k : val)
-(l : Z)
+(l : val)
 (key : list Z)
 (KV : val)
 (h1:hmacabs)
-(KL1 : l = Zlength key)
+(*(KL1 : l = Zlength key)
 (KL2 : 0 <= l <= Int.max_signed)
-(KL3 : l * 8 < two_p 64)
+(KL3 : l * 8 < two_p 64)*)
 (ctx' : name _ctx)
 (key' : name _key)
 (len' : name _len)
-(Delta := (initialized _reset 
-       (func_tycontext f_HMAC_Init HmacVarSpecs HmacFunSpecs)))
+(Delta := initialized _reset 
+       (func_tycontext f_HMAC_Init HmacVarSpecs HmacFunSpecs))
+(*  (initialized _i (initialized _j (initialized _reset 
+       (func_tycontext f_HMAC_Init HmacVarSpecs HmacFunSpecs)))))*)
 (PostKeyNull : environ -> mpred)
 (HeqPostKeyNull : PostKeyNull =
                  EX  cb : block,
                  (EX  cofs : int,
                   (EX  pad : val,
                    (EX  r : Z,
+                    (EX  ctxkey : val,
+                     PROP  (c = Vptr cb cofs /\ (r = 0 \/ r = 1))
+                     LOCAL  (`(eq (Vint (Int.repr r))) (eval_id _reset);
+                     `(eq pad) (eval_var _pad (tarray tuchar 64));
+                     `(eq c) (eval_id _ctx); `(eq k) (eval_id _key);
+                     `(eq l) (eval_id _len);
+                     `(eq ctxkey) (eval_var _ctx_key (tarray tuchar 64));
+                     `(eq KV) (eval_var sha._K256 (tarray tuint 64)))
+                     SEP  (`(data_at_ Tsh (tarray tuchar 64) pad);
+                     `(initPostKeyNullConditional l r c k h1 key ctxkey);
+                     `(K_vector KV))))))),
+@semax Espec (initialized _reset Delta)
+  (PROP  ()
+   LOCAL  (`(eq (Vint (Int.repr 0))) (eval_id _reset);
+   `(eq c) (eval_id _ctx); `(eq k) (eval_id _key); `(eq l) (eval_id _len);
+   `(eq KV) (eval_var sha._K256 (tarray tuint 64)))
+   SEP 
+   (`(data_at_ Tsh (tarray tuchar 64)) (eval_var _pad (tarray tuchar 64));
+   `(data_at_ Tsh (tarray tuchar 64)) (eval_var _ctx_key (tarray tuchar 64));
+   `(K_vector KV); `(initPre l c k h1 key)))
+  (Sifthenelse
+     (Ebinop One (Etempvar _key (tptr tuchar))
+        (Ecast (Econst_int (Int.repr 0) tint) (tptr tvoid)) tint)
+     (Ssequence (Sset _reset (Econst_int (Int.repr 1) tint))
+        (Ssequence (Sset _j (Econst_int (Int.repr 64) tint))
+           (Sifthenelse
+              (Ebinop Olt (Etempvar _j tint) (Etempvar _len tint) tint)
+              (Ssequence
+                 (Scall None
+                    (Evar _SHA256_Init
+                       (Tfunction (Tcons (tptr t_struct_SHA256state_st) Tnil)
+                          tvoid cc_default))
+                    [Eaddrof
+                       (Efield
+                          (Ederef (Etempvar _ctx (tptr t_struct_hmac_ctx_st))
+                             t_struct_hmac_ctx_st) _md_ctx
+                          t_struct_SHA256state_st)
+                       (tptr t_struct_SHA256state_st)])
+                 (Ssequence
+                    (Scall None
+                       (Evar _SHA256_Update
+                          (Tfunction
+                             (Tcons (tptr t_struct_SHA256state_st)
+                                (Tcons (tptr tvoid) (Tcons tuint Tnil)))
+                             tvoid cc_default))
+                       [Eaddrof
+                          (Efield
+                             (Ederef
+                                (Etempvar _ctx (tptr t_struct_hmac_ctx_st))
+                                t_struct_hmac_ctx_st) _md_ctx
+                             t_struct_SHA256state_st)
+                          (tptr t_struct_SHA256state_st);
+                       Etempvar _key (tptr tuchar); Etempvar _len tint])
+                    (Ssequence
+                       (Scall None
+                          (Evar _SHA256_Final
+                             (Tfunction
+                                (Tcons (tptr tuchar)
+                                   (Tcons (tptr t_struct_SHA256state_st) Tnil))
+                                tvoid cc_default))
+                          [Evar _ctx_key (tarray tuchar 64);
+                          Eaddrof
+                            (Efield
+                               (Ederef
+                                  (Etempvar _ctx (tptr t_struct_hmac_ctx_st))
+                                  t_struct_hmac_ctx_st) _md_ctx
+                               t_struct_SHA256state_st)
+                            (tptr t_struct_SHA256state_st)])
+                       (Scall None
+                          (Evar _memset
+                             (Tfunction
+                                (Tcons (tptr tvoid)
+                                   (Tcons tint (Tcons tuint Tnil)))
+                                (tptr tvoid) cc_default))
+                          [Eaddrof
+                             (Ederef
+                                (Ebinop Oadd
+                                   (Evar _ctx_key (tarray tuchar 64))
+                                   (Econst_int (Int.repr 32) tint)
+                                   (tptr tuchar)) tuchar) (tptr tuchar);
+                          Econst_int (Int.repr 0) tint;
+                          Econst_int (Int.repr 32) tint]))))
+              (Ssequence
+                 (Scall None
+                    (Evar _memcpy
+                       (Tfunction
+                          (Tcons (tptr tvoid)
+                             (Tcons (tptr tvoid) (Tcons tuint Tnil)))
+                          (tptr tvoid) cc_default))
+                    [Evar _ctx_key (tarray tuchar 64);
+                    Etempvar _key (tptr tuchar); Etempvar _len tint])
+                 (Scall None
+                    (Evar _memset
+                       (Tfunction
+                          (Tcons (tptr tvoid) (Tcons tint (Tcons tuint Tnil)))
+                          (tptr tvoid) cc_default))
+                    [Eaddrof
+                       (Ederef
+                          (Ebinop Oadd (Evar _ctx_key (tarray tuchar 64))
+                             (Etempvar _len tint) (tptr tuchar)) tuchar)
+                       (tptr tuchar); Econst_int (Int.repr 0) tint;
+                    Ebinop Osub (Econst_int (Int.repr 64) tuint)
+                      (Etempvar _len tint) tuint]))))) Sskip)
+  (normal_ret_assert PostKeyNull).
+(*
+(HeqPostKeyNull : PostKeyNull =
+                 EX  cb : block,
+                 (EX  cofs : int,
+                  (EX  pad : val,
+                   (EX  r : Z, EX ctxkey:val,
                     PROP  (c = Vptr cb cofs /\ (r=0 \/ r=1))
                     LOCAL  (`(eq (Vint (Int.repr r))) (eval_id _reset);
                     `(eq pad) (eval_var _pad (tarray tuchar 64));
                     `(eq c) (eval_id _ctx); `(eq k) (eval_id _key);
                     `(eq (Vint (Int.repr l))) (eval_id _len);
+                    `(eq ctxkey) (eval_var _ctx_key (tarray tuchar 64));
                     `(eq KV) (eval_var sha._K256 (tarray tuint 64)))
                     SEP  (`(data_at_ Tsh (tarray tuchar 64) pad);
-                    `(initPostKeyNullConditional r c k h1 key);
+                    `(initPostKeyNullConditional r c k h1 key ctxkey);
                     `(K_vector KV)))))),
 @semax Espec Delta
   (PROP  ()
@@ -64,7 +198,9 @@ Lemma hmac_init_part1: forall
    `(eq KV) (eval_var sha._K256 (tarray tuint 64)))
    SEP 
    (`(data_at_ Tsh (tarray tuchar 64)) (eval_var _pad (tarray tuchar 64));
+   `(data_at_ Tsh (tarray tuchar 64)) (eval_var _ctx_key (tarray tuchar 64));
    `(K_vector KV); `(initPre c k h1 key)))
+   
      (Sifthenelse
         (Ebinop One (Etempvar _key (tptr tuchar))
            (Ecast (Econst_int (Int.repr 0) tint) (tptr tvoid)) tint)
@@ -107,11 +243,7 @@ Lemma hmac_init_part1: forall
                                    (Tcons (tptr tuchar)
                                       (Tcons (tptr t_struct_SHA256state_st)
                                          Tnil)) tvoid cc_default))
-                             [Efield
-                                (Ederef
-                                   (Etempvar _ctx (tptr t_struct_hmac_ctx_st))
-                                   t_struct_hmac_ctx_st) _key
-                                (tarray tuchar 64);
+                             [Evar _ctx_key (tarray tuchar 64);
                              Eaddrof
                                (Efield
                                   (Ederef
@@ -120,33 +252,20 @@ Lemma hmac_init_part1: forall
                                      t_struct_hmac_ctx_st) _md_ctx
                                   t_struct_SHA256state_st)
                                (tptr t_struct_SHA256state_st)])
-                          (Ssequence
-                             (Scall None
-                                (Evar _memset
-                                   (Tfunction
-                                      (Tcons (tptr tvoid)
-                                         (Tcons tint (Tcons tuint Tnil)))
-                                      (tptr tvoid) cc_default))
-                                [Eaddrof
-                                   (Ederef
-                                      (Ebinop Oadd
-                                         (Efield
-                                            (Ederef
-                                               (Etempvar _ctx
-                                                  (tptr t_struct_hmac_ctx_st))
-                                               t_struct_hmac_ctx_st) _key
-                                            (tarray tuchar 64))
-                                         (Econst_int (Int.repr 32) tint)
-                                         (tptr tuchar)) tuchar) (tptr tuchar);
-                                Econst_int (Int.repr 0) tint;
-                                Econst_int (Int.repr 32) tint])
-                             (Sassign
-                                (Efield
-                                   (Ederef
-                                      (Etempvar _ctx
-                                         (tptr t_struct_hmac_ctx_st))
-                                      t_struct_hmac_ctx_st) _key_length tuint)
-                                (Econst_int (Int.repr 32) tint))))))
+                          (Scall None
+                             (Evar _memset
+                                (Tfunction
+                                   (Tcons (tptr tvoid)
+                                      (Tcons tint (Tcons tuint Tnil)))
+                                   (tptr tvoid) cc_default))
+                             [Eaddrof
+                                (Ederef
+                                   (Ebinop Oadd
+                                      (Evar _ctx_key (tarray tuchar 64))
+                                      (Econst_int (Int.repr 32) tint)
+                                      (tptr tuchar)) tuchar) (tptr tuchar);
+                             Econst_int (Int.repr 0) tint;
+                             Econst_int (Int.repr 32) tint]))))
                  (Ssequence
                     (Scall None
                        (Evar _memcpy
@@ -154,75 +273,73 @@ Lemma hmac_init_part1: forall
                              (Tcons (tptr tvoid)
                                 (Tcons (tptr tvoid) (Tcons tuint Tnil)))
                              (tptr tvoid) cc_default))
-                       [Efield
-                          (Ederef (Etempvar _ctx (tptr t_struct_hmac_ctx_st))
-                             t_struct_hmac_ctx_st) _key (tarray tuchar 64);
+                       [Evar _ctx_key (tarray tuchar 64);
                        Etempvar _key (tptr tuchar); Etempvar _len tint])
-                    (Ssequence
-                       (Scall None
-                          (Evar _memset
-                             (Tfunction
-                                (Tcons (tptr tvoid)
-                                   (Tcons tint (Tcons tuint Tnil)))
-                                (tptr tvoid) cc_default))
-                          [Eaddrof
-                             (Ederef
-                                (Ebinop Oadd
-                                   (Efield
-                                      (Ederef
-                                         (Etempvar _ctx
-                                            (tptr t_struct_hmac_ctx_st))
-                                         t_struct_hmac_ctx_st) _key
-                                      (tarray tuchar 64))
-                                   (Etempvar _len tint) (tptr tuchar)) tuchar)
-                             (tptr tuchar); Econst_int (Int.repr 0) tint;
-                          Ebinop Osub (Econst_int (Int.repr 64) tuint)
-                            (Etempvar _len tint) tuint])
-                       (Sassign
-                          (Efield
-                             (Ederef
-                                (Etempvar _ctx (tptr t_struct_hmac_ctx_st))
-                                t_struct_hmac_ctx_st) _key_length tuint)
-                          (Etempvar _len tint))))))) Sskip)
+                    (Scall None
+                       (Evar _memset
+                          (Tfunction
+                             (Tcons (tptr tvoid)
+                                (Tcons tint (Tcons tuint Tnil))) (tptr tvoid)
+                             cc_default))
+                       [Eaddrof
+                          (Ederef
+                             (Ebinop Oadd (Evar _ctx_key (tarray tuchar 64))
+                                (Etempvar _len tint) (tptr tuchar)) tuchar)
+                          (tptr tuchar); Econst_int (Int.repr 0) tint;
+                       Ebinop Osub (Econst_int (Int.repr 64) tuint)
+                         (Etempvar _len tint) tuint]))))) Sskip)
   (normal_ret_assert PostKeyNull).
+*)
 Proof. intros. subst Delta. abbreviate_semax.
 forward_if PostKeyNull.
   { (* THEN*)
-    simpl. 
-    unfold force_val2, force_val1; simpl. 
-    eapply semax_pre with (P':= EX cb:_, EX cofs:_, EX kb:_, EX kofs:_, EX pad:_,
-      (PROP  (c=Vptr cb cofs /\ k=Vptr kb kofs /\ Forall isbyteZ key)
+    simpl.  
+    unfold force_val2, force_val1; simpl.
+    eapply semax_pre with (P':= EX cb:_, EX cofs:_, EX kb:_, EX kofs:_, 
+      EX pad:_, EX ctxkey:_, EX  ll : Z,
+      (PROP  (c=Vptr cb cofs /\ k=Vptr kb kofs /\ Forall isbyteZ key /\
+              has_lengthK ll key /\ l = Vint (Int.repr ll)) 
        LOCAL 
          (`(eq (Vint (Int.repr 0))) (eval_id _reset);
           `(eq pad) (eval_var _pad (tarray tuchar 64)); `(eq c) (eval_id _ctx);
-          `(eq k) (eval_id _key); `(eq (Vint (Int.repr l))) (eval_id _len);
+          `(eq k) (eval_id _key); `(eq  l) (eval_id _len);
+          `(eq ctxkey) (eval_var _ctx_key (tarray tuchar 64));
           `(eq KV) (eval_var sha._K256 (tarray tuint 64)))
       SEP  (
           `(data_at_ Tsh (tarray tuchar 64) pad);
           `(data_at_ Tsh t_struct_hmac_ctx_st (Vptr cb cofs));
           `(K_vector KV);
-          `(array_at tuchar Tsh (tuchars (map Int.repr key)) 0 (Zlength key) k)))).
+          `(array_at tuchar Tsh (tuchars (map Int.repr key)) 0 (Zlength key) k);
+          `(data_at_ Tsh (tarray tuchar 64) ctxkey)))).
       entailer.
-      destruct key'; try contradiction.
+      destruct key'; try contradiction. simpl in *.
       (*key' is integer, ie Null*)
-        simpl in *. subst i. unfold Int.zero in *. simpl in *.
-        unfold Vfalse in H0. inversion H0.
+       { simpl in *. subst i. unfold Int.zero in *. simpl in *.
+        unfold Vfalse in H0. inversion H0. }
       (*key' is ptr*)
-        simpl in *. rewrite (data_at__isptr _ t_struct_hmac_ctx_st). 
-        entailer. apply isptrD in Pctx'. destruct Pctx' as [cb [cofs CB]]. subst ctx'.
+       { simpl in *. rewrite (data_at__isptr _ t_struct_hmac_ctx_st). 
+        entailer. clear HeqPostKeyNull.
+        apply isptrD in H5. destruct H5 as [cb [cofs CB]]. subst ctx'.
         apply exp_right with (x:=cb).
         apply exp_right with (x:=cofs).
         apply exp_right with (x:=b).
         apply exp_right with (x:=i).
         apply exp_right with (x:=eval_var _pad (tarray tuchar 64) rho).
+        apply exp_right with (x:=eval_var _ctx_key (tarray tuchar 64) rho).
+        apply exp_right with (x:=ll).
         entailer. cancel.
         unfold data_block. entailer.
+       }
     apply extract_exists_pre. intros cb. 
     apply extract_exists_pre. intros cofs.  
     apply extract_exists_pre. intros kb. 
     apply extract_exists_pre. intros kofs.  
     apply extract_exists_pre. intros pad.  
-    normalize. subst c k. rename H1 into isbyte_key. (*subst PostKeyNull.*)
+    apply extract_exists_pre. intros ctxkey.  
+    apply extract_exists_pre. intros ll.  
+    normalize. subst c k l. rename H1 into isbyte_key. 
+    rename H2 into KL. rename ll into l. (*subst PostKeyNull.*)
+    destruct KL as [KL1 [KL2 KL3]].
 
     forward. (*reset =1 *) (*qinxiang: here, forward now intoduces an essentially 
       unnecessary x:val, together with a term `(eq (Vint (Int.repr 0))) `x; in LOCAL*) 
@@ -235,15 +352,18 @@ forward_if PostKeyNull.
        `(eq (Vint (Int.repr 1))) (eval_id _reset);
        `(eq pad) (eval_var _pad (tarray tuchar 64)); `(eq (Vptr cb cofs)) (eval_id _ctx);
        `(eq (Vptr kb kofs)) (eval_id _key); `(eq (Vint (Int.repr l))) (eval_id _len);
+       `(eq ctxkey) (eval_var _ctx_key (tarray tuchar 64));
        `(eq KV) (eval_var sha._K256 (tarray tuint 64)))
       SEP  (`(data_at_ Tsh (tarray tuchar 64) pad);
-            `(data_at Tsh t_struct_hmac_ctx_st (keyedHMS key) (Vptr cb cofs));
+            `(data_at Tsh t_struct_hmac_ctx_st keyedHMS (Vptr cb cofs));
            `(array_at tuchar Tsh (tuchars (map Int.repr key)) 0 (Zlength key)
              (Vptr kb kofs));
+           `(data_at Tsh (tarray tuchar 64) (map Vint (map Int.repr (HMAC_SHA256.mkKey key)))
+                ctxkey);
           `(K_vector KV))) as PostIf_j_Len.
 
     forward_if PostIf_j_Len. 
-    { (* j < len*)
+    { (* j < len*) 
       eapply semax_pre with (P':=
        (PROP  (64 < l)
         LOCAL 
@@ -251,30 +371,33 @@ forward_if PostKeyNull.
           `eq (eval_id _reset) `(Vint (Int.repr 1));
           `(eq pad) (eval_var _pad (tarray tuchar 64)); `(eq (Vptr cb cofs)) (eval_id _ctx);
           `(eq (Vptr kb kofs)) (eval_id _key); `(eq (Vint (Int.repr l))) (eval_id _len);
+                  `(eq ctxkey) (eval_var _ctx_key (tarray tuchar 64));
           `(eq KV) (eval_var sha._K256 (tarray tuint 64)))
         SEP  (`(data_at_ Tsh (tarray tuchar 64) pad);
-              `(data_at_ Tsh t_struct_hmac_ctx_st (Vptr cb cofs));
-              `(K_vector KV);
+              `(data_at Tsh t_struct_hmac_ctx_st (default_val t_struct_hmac_ctx_st) (Vptr cb cofs));
+              `(K_vector KV); `(data_at_ Tsh (tarray tuchar 64) ctxkey);
               `(array_at tuchar Tsh (tuchars (map Int.repr key)) 0 (Zlength key) (Vptr kb kofs))))).
-        entailer. 
+        entailer. cancel. 
       normalize. rename H into lt_64_l.
-      clear x. (*here's where we can finally eliminate the spurious x*) 
+      clear x. (*here's where we can finally elimnate the spurious x*) 
 
       (*call to SHA256_init*)
-      eapply semax_seq'.
-      frame_SEP 1.
-      unfold data_at_.
       unfold_data_at 1%nat.
       rewrite (field_at_data_at Tsh t_struct_hmac_ctx_st [_md_ctx]); try reflexivity.
       normalize. 
       rename H into SCc. rename H0 into ACc.
+      eapply semax_seq'.
+      frame_SEP 0 1 2.
+(*      unfold data_at_.
+      unfold_data_at 1%nat.*)(*
+      rewrite (field_at_data_at Tsh t_struct_hmac_ctx_st [_md_ctx]); try reflexivity.
+      normalize. 
+      rename H into SCc. rename H0 into ACc.*)
       (*rewrite isptr_c; simpl.*)
-      (*rewrite at_offset'_eq.
-      2: rewrite isptr_c; simpl; rewrite Int.add_zero; reflexivity.*)
+      rewrite at_offset'_eq.
+      2: simpl; rewrite Int.add_zero; reflexivity.
       forward_call (Vptr cb cofs). 
       { assert (FR: Frame = [
-        `(field_at Tsh t_struct_hmac_ctx_st [_key_length] Vundef (Vptr cb cofs));
-        `(field_at Tsh t_struct_hmac_ctx_st [_key] [] (Vptr cb cofs));
         `(field_at Tsh t_struct_hmac_ctx_st [_o_ctx]
                ([], (Vundef, (Vundef, ([], Vundef)))) (Vptr cb cofs));
         `(field_at Tsh t_struct_hmac_ctx_st [_i_ctx]
@@ -292,7 +415,7 @@ forward_if PostKeyNull.
       rewrite isptr_k in H, H0. *) simpl in H, H0. rewrite Zplus_0_r in H.
       rename H into OIR_kofs. rename H0 into OIR_kofs_key.
       eapply semax_seq'.
-      frame_SEP 8 0 2.
+      frame_SEP 6 0 2.
       remember (init_s256abs, key, Vptr cb cofs,
                 Vptr kb kofs, Tsh, l, KV) as WITNESS.
       forward_call WITNESS.
@@ -314,12 +437,13 @@ forward_if PostKeyNull.
      apply semax_pre with (P':=
       EX  xx : s256abs,
   (PROP  ()
-   LOCAL  (tc_environ Delta; 
+   LOCAL  (tc_environ Delta;
    `(eq (Vint (Int.repr 64))) (eval_id _j);
    `(eq (Vint (Int.repr 1))) (eval_id _reset);
    `(eq pad) (eval_var _pad (tarray tuchar 64));
    `(eq (Vptr cb cofs)) (eval_id _ctx); `(eq (Vptr kb kofs)) (eval_id _key);
    `(eq (Vint (Int.repr l))) (eval_id _len);
+   `(eq ctxkey) (eval_var _ctx_key (tarray tuchar 64));
    `(eq KV) (eval_var sha._K256 (tarray tuint 64)))
    SEP 
    (`(fun a : environ =>
@@ -329,25 +453,25 @@ forward_if PostKeyNull.
        `(data_block Tsh key (Vptr kb kofs)))) a) globals_only;
    `(array_at tuchar Tsh (fun i : Z => tuchars (map Int.repr key) (i + l)) 0
        (Zlength key - l) (Vptr kb (Int.add kofs (Int.repr l))));
-   `(field_at Tsh t_struct_hmac_ctx_st [_key_length] Vundef (Vptr cb cofs));
-   `(field_at Tsh t_struct_hmac_ctx_st [_key] [] (Vptr cb cofs));
    `(field_at Tsh t_struct_hmac_ctx_st [_o_ctx]
        ([], (Vundef, (Vundef, ([], Vundef)))) (Vptr cb cofs));
    `(field_at Tsh t_struct_hmac_ctx_st [_i_ctx]
        ([], (Vundef, (Vundef, ([], Vundef)))) (Vptr cb cofs));
-   `(data_at_ Tsh (tarray tuchar 64) pad)))).
+   `(data_at_ Tsh (tarray tuchar 64) pad);
+   `(data_at Tsh (Tarray tuchar 64 noattr)
+       (default_val (Tarray tuchar 64 noattr)) ctxkey)))).
        entailer. rename x into a. apply (exp_right a).
        entailer.
-   apply extract_exists_pre. intros ctxSha. simpl. normalize. simpl.
-
+   apply extract_exists_pre. intros ctxSha. simpl. rewrite data_at_isptr. normalize. simpl.
+   normalize. apply isptrD in H0. destruct H0 as [ckb [ckofs CTK]]; subst ctxkey. simpl.
    (*call Final*)
-   rewrite (field_at_data_at Tsh t_struct_hmac_ctx_st [_key]); try reflexivity.
+   (*rewrite (field_at_data_at Tsh t_struct_hmac_ctx_st [_key]); try reflexivity.
    normalize. 
    rewrite at_offset'_eq.
      2: simpl; rewrite Int.add_zero; reflexivity.
    unfold nested_field_offset2, nested_field_type2; simpl.
-   unfold tarray.
-   erewrite (data_at_array_at Tsh tuchar 64 noattr []).
+   unfold tarray.*)
+   unfold tarray. erewrite (data_at_array_at Tsh tuchar 64 noattr []).
      2: apply JMeq.JMeq_refl. 
      2: omega.
      2: reflexivity. 
@@ -355,7 +479,7 @@ forward_if PostKeyNull.
    normalize.
    eapply semax_seq'.
    frame_SEP 2 3 0.
-   remember (ctxSha, Vptr cb (Int.add cofs (Int.repr 328)),
+   remember (ctxSha, Vptr ckb ckofs,
              Vptr cb cofs, Tsh, Tsh, KV) as WITNESS.
    forward_call WITNESS.
      { assert (FR: Frame = []).
@@ -369,98 +493,59 @@ forward_if PostKeyNull.
    (*call memset*)
    (* doing this: eapply semax_seq'. frame_SEP 3. requires us to do the swap fun a=> vs EX
       after the call, which leaves a state that still doesn't nicely normalize *)
-   remember (Tsh, Vptr cb (Int.add cofs (Int.repr 360)), 32, Int.zero) as WITNESS.
+   remember (Tsh, Vptr ckb (Int.add ckofs (Int.repr 32)), 32, Int.zero) as WITNESS.
    forward_call WITNESS.
      { assert (FR: Frame = [`(K_vector KV);
-         `(data_at_ Tsh sha.t_struct_SHA256state_st (Vptr cb cofs));
-         `(data_block Tsh (sha_finish ctxSha) (Vptr cb (Int.add cofs (Int.repr 328))));
-         `(data_block Tsh key (Vptr kb kofs));
-         `(array_at tuchar Tsh (fun i : Z => tuchars (map Int.repr key) (i + l)) 0
-              (Zlength key - l) (offset_val (Int.repr l) (Vptr kb kofs)));
-         `(field_at Tsh t_struct_hmac_ctx_st [_key_length] Vundef (Vptr cb cofs));
-         `(field_at Tsh t_struct_hmac_ctx_st [_o_ctx]
-              ([], (Vundef, (Vundef, ([], Vundef)))) (Vptr cb cofs));
-         `(field_at Tsh t_struct_hmac_ctx_st [_i_ctx]
-              ([], (Vundef, (Vundef, ([], Vundef)))) (Vptr cb cofs));
-(*         `(data_at_ Tsh t_struct_SHA256state_st sha);*)
-         `(data_at_ Tsh (Tarray tuchar 64 noattr) pad)]).
+       `(data_at_ Tsh sha.t_struct_SHA256state_st (Vptr cb cofs));
+       `(data_block Tsh (sha_finish ctxSha) (Vptr ckb ckofs));
+       `(data_block Tsh key (Vptr kb kofs));
+       `(array_at tuchar Tsh (fun i : Z => tuchars (map Int.repr key) (i + l)) 0
+           (Zlength key - l) (Vptr kb (Int.add kofs (Int.repr l))));
+       `(field_at Tsh t_struct_hmac_ctx_st [_o_ctx]
+           ([], (Vundef, (Vundef, ([], Vundef)))) (Vptr cb cofs));
+       `(field_at Tsh t_struct_hmac_ctx_st [_i_ctx]
+           ([], (Vundef, (Vundef, ([], Vundef)))) (Vptr cb cofs));
+       `(data_at_ Tsh (Tarray tuchar 64 noattr) pad)]).
          subst Frame. reflexivity.
        rewrite FR. clear FR Frame.   
-       entailer. cancel. 
-       rewrite memory_block_array_tuchar'. cancel. trivial. omega.
+       entailer. rewrite <- H3. simpl. rewrite Int.add_zero, Int.mul_commut, Int.mul_one.
+       rewrite memory_block_array_tuchar'.
+       apply andp_right. apply prop_right; auto. 
+       cancel. trivial. omega.
      } 
-     after_call. subst WITNESS. normalize. subst retval0. 
-   (*swap fun a=> with EX
-   apply semax_pre with (P':=
-    EX  x : val,
-  (PROP  ()
-   LOCAL  (tc_environ Delta; tc_environ Delta; tc_environ Delta;
-   tc_environ Delta; `(eq (Vint (Int.repr 1))) (eval_id _reset);
-   `(eq sha) (eval_var _sha_ctx t_struct_SHA256state_st);
-   `(eq pad) (eval_var _pad (Tarray tuchar 64 noattr));
-   `(eq (Vptr cb cofs)) (eval_id _ctx); `(eq k) (eval_id _key);
-   `(eq (Vint (Int.repr l))) (eval_id _len);
-   `(eq KV) (eval_var sha._K256 (Tarray tuint 64 noattr)))
-   SEP 
-   (fun a : environ =>
-    `(fun x0 : environ =>
-      local (`(eq (Vptr cb (Int.add cofs (Int.repr 360)))) retval) x0 &&
-      `(array_at tuchar Tsh (fun _ : Z => Vint Int.zero) 0 32
-          (Vptr cb (Int.add cofs (Int.repr 360)))) x0)
-      (fun rho : environ => env_set (globals_only rho) ret_temp x) a;
-   `(K_vector KV);
-   `(data_at_ Tsh sha.t_struct_SHA256state_st (Vptr cb cofs));
-   `(data_block Tsh (sha_finish mdSha)
-       (Vptr cb (Int.add cofs (Int.repr 328))));
-   `(data_block Tsh key (Vptr kb kofs));
-   `(array_at tuchar Tsh (fun i : Z => tuchars (map Int.repr key) (i + l)) 0
-       (Zlength key - l) (offset_val (Int.repr l) k));
-   `(field_at Tsh t_struct_hmac_ctx_st [_key_length] Vundef (Vptr cb cofs));
-   `(field_at Tsh t_struct_hmac_ctx_st [_o_ctx]
-       ([], (Vundef, (Vundef, ([], Vundef)))) (Vptr cb cofs));
-   `(field_at Tsh t_struct_hmac_ctx_st [_i_ctx]
-       ([], (Vundef, (Vundef, ([], Vundef)))) (Vptr cb cofs));
-   `(data_at_ Tsh t_struct_SHA256state_st sha);
-   `(data_at_ Tsh (Tarray tuchar 64 noattr) pad)))).
-    entailer.
-    apply exp_right with (x:=Vptr cb (Int.add cofs (Int.repr 360))).
-    entailer.
-   apply extract_exists_pre. intros x. simpl. normalize.
-     unfold local. simpl. red. normalize.*)
-
-   forward. (*ctx->key_length=32*)
-
+     after_call. subst WITNESS. 
    subst PostIf_j_Len.
    entailer. 
-   cancel.
+   rewrite Z.sub_diag, array_at_emp. 
    unfold data_block. entailer. cancel. 
    unfold data_at_.
    destruct (zlt 64 (Zlength key)). 2: omega.
    unfold_data_at 2%nat.
    cancel. 
-   rewrite (field_at_data_at Tsh t_struct_hmac_ctx_st [_key]); try reflexivity.
+(*   rewrite (field_at_data_at Tsh t_struct_hmac_ctx_st [_key]); try reflexivity.
      entailer.
      rewrite at_offset'_eq.
      2: simpl; rewrite Int.add_zero; reflexivity.
      unfold nested_field_offset2, nested_field_type2; simpl.
-     unfold tarray.
+     unfold tarray.*)
      erewrite (data_at_array_at Tsh tuchar 64 noattr).
      2: apply JMeq.JMeq_refl. 
      2: omega.
-     2: reflexivity. 
+     2: reflexivity.
+     
      erewrite (split_offset_array_at _ _ _ 0 32 64); try reflexivity. 2: omega.
-     entailer. unfold offset_val. rewrite Int.add_assoc.
+     entailer. unfold offset_val. (*rewrite Int.add_assoc.
         assert (I360: Int.add (Int.repr 328) (Int.repr 32) = Int.repr 360).
           reflexivity. 
-        rewrite I360; clear I360.  simpl.
+        rewrite I360; clear I360. *) simpl.
      assert (LengthShaFinish: Zlength (sha_finish ctxSha) = 32).
                  unfold sha_finish. destruct ctxSha.
         rewrite <- functional_prog.SHA_256'_eq, Zlength_correct, length_SHA256'. reflexivity.
      rewrite array_at_ext with (f':= fun i : Z =>
          ZnthV tuchar (map Vint (map Int.repr (HMAC_SHA256.mkKey key))) (i + 32)).
-     Focus 2. intros. unfold ZnthV. if_tac. omega.
+     Focus 2. intros i XX. unfold ZnthV. if_tac. omega.
               assert (Z32: (Z.to_nat i < 32)%nat).
-                  clear - H7; destruct H7 as [XX YY]. rewrite Z2Nat.inj_lt in YY.
+                  clear - XX; destruct XX as [XX YY]. rewrite Z2Nat.inj_lt in YY.
                   apply YY. omega. omega.
                unfold HMAC_SHA256.mkKey. simpl.
                assert (Kgt: Zlength key > 64) by omega.
@@ -470,7 +555,7 @@ forward_if PostKeyNull.
                  remember (HMAC_SHA256.Nlist 0 (SHA256.BlockSize - SHA256.DigestLength)) as NL.
                  simpl.
                  assert (I: (Z.to_nat (i + 32) - 32)%nat = Z.to_nat i).
-                             destruct H7. specialize (Z2Nat.inj_sub (i+32) 32).
+                             destruct XX. specialize (Z2Nat.inj_sub (i+32) 32).
                              simpl; intros HH. rewrite <- HH, Zplus_comm, Zminus_plus. trivial.
                              omega. 
                  unfold SHA256.DigestLength. rewrite I. subst NL. 
@@ -486,9 +571,9 @@ forward_if PostKeyNull.
      cancel.
      rewrite LengthShaFinish.
      rewrite array_at_ext with (f':=ZnthV tuchar (map Vint (map Int.repr (HMAC_SHA256.mkKey key)))).
-     Focus 2. unfold tuchars, sha_finish; intros. destruct ctxSha. simpl.
+     Focus 2. unfold tuchars, sha_finish; intros i XX. destruct ctxSha. simpl.
               assert (Z32: (Z.to_nat i < 32)%nat).
-                  clear - H7; destruct H7 as [XX YY]. rewrite Z2Nat.inj_lt in YY.
+                  clear - XX; destruct XX as [XX YY]. rewrite Z2Nat.inj_lt in YY.
                   apply YY. omega. omega.    
               unfold ZnthV. destruct (zlt i 0). omega.   
               rewrite nth_map' with (d':=Int.zero). rewrite nth_map' with (d':=Z0). 
@@ -498,7 +583,7 @@ forward_if PostKeyNull.
               apply Zgt_is_gt_bool in Z6; rewrite Z6.
               unfold HMAC_SHA256.zeroPad.
               rewrite <- functional_prog.SHA_256'_eq.
-              rewrite app_nth1. inversion H. subst. clear H. simpl in *.
+              rewrite app_nth1. inversion H. clear H. simpl in *.
                       rewrite <- H17. rewrite firstn_precise. trivial.
                       rewrite Zlength_correct, Nat2Z.id; trivial.
               rewrite length_SHA256'; trivial.
@@ -508,12 +593,7 @@ forward_if PostKeyNull.
               rewrite map_length, <- functional_prog.SHA_256'_eq, length_SHA256'. trivial. 
      cancel.
    rewrite (field_at_data_at Tsh t_struct_hmac_ctx_st [_md_ctx]); try reflexivity.
-     normalize. 
-     rewrite at_offset'_eq.
-     2: simpl; rewrite Int.add_zero; reflexivity.
-     unfold nested_field_offset2, nested_field_type2; simpl. rewrite Int.add_zero.
-     cancel. rewrite <- Zminus_diag_reverse. rewrite array_at_emp. normalize.
-     destruct (zlt 64 (Zlength key)). trivial. omega.
+     entailer.
    } 
 
    { (* j >= len*)
@@ -521,14 +601,17 @@ forward_if PostKeyNull.
        (PROP  (64 >= l)
         LOCAL 
          (`(eq (Vint (Int.repr 64))) (eval_id _j);
-          `eq (eval_id _reset) `(Vint (Int.repr 1));
-          `(eq pad) (eval_var _pad (tarray tuchar 64)); `(eq (Vptr cb cofs)) (eval_id _ctx);
-          `(eq (Vptr kb kofs)) (eval_id _key); `(eq (Vint (Int.repr l))) (eval_id _len);
+          `(eq (Vint (Int.repr 1))) (eval_id _reset); 
+          `(eq pad) (eval_var _pad (tarray tuchar 64));
+          `(eq (Vptr cb cofs)) (eval_id _ctx); `(eq (Vptr kb kofs)) (eval_id _key);
+          `(eq (Vint (Int.repr l))) (eval_id _len);
+          `(eq ctxkey) (eval_var _ctx_key (tarray tuchar 64));
           `(eq KV) (eval_var sha._K256 (tarray tuint 64)))
         SEP  (`(data_at_ Tsh (tarray tuchar 64) pad);
-              `(data_at Tsh t_struct_hmac_ctx_st (default_val t_struct_hmac_ctx_st) (Vptr cb cofs));
-              `(K_vector KV);
-              `(array_at tuchar Tsh (tuchars (map Int.repr key)) 0 (Zlength key) (Vptr kb kofs))))).
+              `(data_at_ Tsh t_struct_hmac_ctx_st (Vptr cb cofs)); `(K_vector KV);
+              `(array_at tuchar Tsh (tuchars (map Int.repr key)) 0 (Zlength key)
+                   (Vptr kb kofs));
+              `(data_at Tsh (tarray tuchar 64) (default_val (tarray tuchar 64)) ctxkey)))).
         entailer. 
      normalize. rename H into ge_64_l. 
      clear x. (*again, remove spurious x*)
@@ -536,13 +619,13 @@ forward_if PostKeyNull.
      (*call to memcpy*)
      (*eapply semax_seq'.*)
      focus_SEP 1 3.
-     (*unfold data_at_. *)
-     unfold_data_at 1%nat.
-     rewrite (field_at_data_at Tsh t_struct_hmac_ctx_st [_key]); try reflexivity.
-     normalize. 
-     rename H into SCc. rename H0 into ACc.
+     (*unfold_data_at 1%nat.
+     rewrite (field_at_data_at Tsh t_struct_hmac_ctx_st [_key]); try reflexivity.*)
+     rewrite data_at_isptr. normalize. simpl.
+     apply isptrD in H. destruct H as [ckb [ckofs CTK]]; subst ctxkey. simpl.
+     (*rename H into SCc. rename H0 into ACc.
      (*rewrite isptr_c;*) simpl.
-     rewrite at_offset_data_at. unfold nested_field_type2, nested_field_offset2; simpl.
+     rewrite at_offset_data_at. unfold nested_field_type2, nested_field_offset2; simpl.*)
      unfold tarray.
      erewrite data_at_array_at. 2: apply JMeq.JMeq_refl. 2: omega. 2: reflexivity.
      erewrite (split_offset_array_at _ _ _ 0 l 64); try reflexivity. 2: omega.
@@ -550,23 +633,15 @@ forward_if PostKeyNull.
      rename H into OIR0_328. rename H0 into OIR64_328.
 
      unfold tuchars. remember (64 - l) as l64.
-     remember ((Tsh, Tsh), Vptr cb (Int.add cofs (Int.repr 328)), 
+     remember ((Tsh, Tsh), Vptr ckb ckofs, 
              Vptr kb kofs, mkTrep (Tarray tuchar (Zlength key) noattr) 
                      (map Vint (map Int.repr key))) as WITNESS.
      forward_call WITNESS.
      { assert (FR: Frame = [
-        `(array_at tuchar Tsh (fun i : Z => ZnthV tuchar [] (i + l)) 0 l64
-            (offset_val (Int.repr l) (Vptr cb (Int.add cofs (Int.repr 328)))));
-        `(field_at Tsh t_struct_hmac_ctx_st [_key_length] Vundef (Vptr cb cofs));
-        `(field_at Tsh t_struct_hmac_ctx_st [_o_ctx]
-            ([], (Vundef, (Vundef, ([], Vundef)))) (Vptr cb cofs));
-        `(field_at Tsh t_struct_hmac_ctx_st [_i_ctx]
-            ([], (Vundef, (Vundef, ([], Vundef)))) (Vptr cb cofs));
-        `(field_at Tsh t_struct_hmac_ctx_st [_md_ctx]
-            ([], (Vundef, (Vundef, ([], Vundef)))) (Vptr cb cofs));
-        `(data_at_ Tsh (Tarray tuchar 64 noattr) pad);
-        (*`(array_at tuchar Tsh (ZnthV tuchar []) 0 64 pad);*)
-        `(K_vector KV)]).
+         `(array_at tuchar Tsh (fun i : Z => ZnthV tuchar [] (i + l)) 0 l64
+             (offset_val (Int.repr l) (Vptr ckb ckofs)));
+         `(data_at_ Tsh t_struct_hmac_ctx_st (Vptr cb cofs));
+         `(data_at_ Tsh (Tarray tuchar 64 noattr) pad); `(K_vector KV)]).
          subst Frame. reflexivity.
        rewrite FR. clear FR Frame.   
        subst WITNESS. entailer.
@@ -587,12 +662,7 @@ forward_if PostKeyNull.
        apply sepcon_derives.
          erewrite data_at_array_at.
          apply array_lemmas.array_at_ext'. intros. reflexivity. 
-         trivial. omega. reflexivity. (*  unfold cVint, ZnthV; intros.
-         if_tac. omega. 
-              rewrite nth_map' with (d':=Int.zero). trivial.
-              rewrite map_length. clear - H0.
-              rewrite Zlength_correct in H0; destruct H0 as [XX YY].
-              apply Z2Nat.inj_lt in YY; trivial. rewrite Nat2Z.id in YY; trivial. omega.*)
+         trivial. omega. reflexivity. 
        rewrite memory_block_array_tuchar'. cancel.
          reflexivity. omega.
      } 
@@ -600,72 +670,54 @@ forward_if PostKeyNull.
        remember (map Vint (map Int.repr key)) as CONT.
 
    (*call memset*)
-   remember (Tsh, Vptr cb (Int.add cofs (Int.repr (Zlength key + 328))), l64, Int.zero) as WITNESS.
+   remember (Tsh, Vptr ckb (Int.add ckofs (Int.repr (Zlength key))), l64, Int.zero) as WITNESS.
    forward_call WITNESS.
      { assert (FR: Frame = [
-        `(data_at Tsh (Tarray tuchar (Zlength key) noattr)
-              CONT (Vptr cb (Int.add cofs (Int.repr 328))));
-        `(data_at Tsh (Tarray tuchar (Zlength key) noattr)
-              CONT (Vptr kb kofs));
-         (* `(array_at tuchar Tsh CONT 0 l k);
-         `(array_at tuchar Tsh CONT 0 l (Vptr cb (Int.add cofs (Int.repr 328))));*)
-         `(field_at Tsh t_struct_hmac_ctx_st [_key_length] Vundef (Vptr cb cofs));
-         `(field_at Tsh t_struct_hmac_ctx_st [_o_ctx]
-             ([], (Vundef, (Vundef, ([], Vundef)))) (Vptr cb cofs));
-         `(field_at Tsh t_struct_hmac_ctx_st [_i_ctx]
-             ([], (Vundef, (Vundef, ([], Vundef)))) (Vptr cb cofs));
-         `(field_at Tsh t_struct_hmac_ctx_st [_md_ctx]
-             ([], (Vundef, (Vundef, ([], Vundef)))) (Vptr cb cofs));
-         `(data_at_ Tsh (Tarray tuchar 64 noattr) pad);
-         (*`(array_at tuchar Tsh (ZnthV tuchar []) 0 64 pad);*)
-         `(K_vector KV)]).
+            `(data_at Tsh (Tarray tuchar (Zlength key) noattr) CONT (Vptr ckb ckofs));
+            `(data_at Tsh (Tarray tuchar (Zlength key) noattr) CONT (Vptr kb kofs));
+            `(data_at_ Tsh t_struct_hmac_ctx_st (Vptr cb cofs));
+            `(data_at_ Tsh (Tarray tuchar 64 noattr) pad); `(K_vector KV)]).
          subst Frame. reflexivity.
        rewrite FR. clear FR Frame.   
-       subst WITNESS. entailer.
+       subst WITNESS. entailer. rewrite <- H0.
        apply andp_right. apply prop_right.
+         split; trivial.
+         split; trivial.
          clear - KL2; split.
            specialize (initial_world.zlength_nonneg _ key); intros.
            rewrite int_max_unsigned_eq. omega.
-         unfold offset_val. rewrite Zplus_comm. trivial.
-       cancel. rewrite Zplus_comm.
+         unfold offset_val. simpl. rewrite Int.add_zero, Int.mul_commut, Int.mul_one. trivial.
+       cancel. 
        rewrite memory_block_array_tuchar'. cancel. trivial. omega.
      } 
-     after_call. subst WITNESS. normalize. subst retval0. 
+     after_call. subst WITNESS. normalize. 
 
-   forward. (*ctx->key_length=len*)
    subst PostIf_j_Len. entailer. cancel.
    unfold_data_at 3%nat. entailer.
    cancel.
    destruct (zlt 64 (Zlength key)). omega. cancel.  
+   apply andp_right. destruct OIR64_328. apply prop_right. split. trivial. 
+         apply Z.divide_1_l.
+   rewrite sepcon_comm.
    apply sepcon_derives.
-   Focus 2. 
       erewrite data_at_array_at. unfold tuchars. apply derives_refl.
       reflexivity. omega. reflexivity.
-  (*
-   unfold_data_at 1%nat.
-   cancel.*)
-   rewrite (field_at_data_at Tsh t_struct_hmac_ctx_st [_key]); try reflexivity.
-     entailer.
-     rewrite at_offset'_eq.
-     2: simpl; rewrite Int.add_zero; reflexivity.
-     remember (64 - Zlength key) as ZK64. 
-     unfold nested_field_offset2, nested_field_type2; simpl.
-     unfold tarray.
-     erewrite (data_at_array_at Tsh tuchar 64 noattr).
+   remember (64 - Zlength key) as ZK64. 
+     erewrite (data_at_array_at Tsh).
      2: apply JMeq.JMeq_refl. 
      2: omega.
      2: reflexivity. 
      erewrite (split_offset_array_at _ _ _ 0 (Zlength key) 64); try reflexivity. 2: omega.
-     entailer. unfold offset_val. rewrite Int.add_assoc. rewrite add_repr. rewrite (Zplus_comm 328).
+     entailer. unfold offset_val. (*rewrite Int.add_assoc. rewrite add_repr. rewrite (Zplus_comm 328).*)
      rewrite sepcon_comm. 
      assert (F64: false = (Zlength key >? 64)). 
        rewrite Z.gtb_ltb. symmetry. apply Fcore_Zaux.Zlt_bool_false. omega.
      apply sepcon_derives. 
-       erewrite data_at_array_at. 2: apply JMeq.JMeq_refl. 2: omega. 2: reflexivity.
+       (*erewrite data_at_array_at. 2: apply JMeq.JMeq_refl. 2: omega. 2: reflexivity.*)
        apply array_lemmas.array_at_ext'.
-         unfold tuchars, cVint, ZnthV; intros. if_tac. omega.
+         unfold tuchars, cVint, ZnthV; intros i XX. if_tac. omega.
          assert (Z32: (Z.to_nat i < length key)%nat).
-                  clear - H1; destruct H1 as [XX YY]. rewrite Zlength_correct, Z2Nat.inj_lt in YY.
+                  clear - XX; destruct XX as [XX YY]. rewrite Zlength_correct, Z2Nat.inj_lt in YY.
                   rewrite Nat2Z.id in YY; trivial. trivial. omega. 
          apply eq_sym.
          assert (L1: (Z.to_nat i < length (HMAC_SHA256.mkKey key))%nat).
@@ -680,10 +732,10 @@ forward_if PostKeyNull.
          eapply mkKey_left; trivial. 
          rewrite map_length; trivial. rewrite map_length; trivial. 
        apply array_lemmas.array_at_ext'.
-         unfold tuchars, cVint, ZnthV; intros. if_tac. omega.
+         unfold tuchars, cVint, ZnthV; intros i XX. if_tac. omega.
          assert (L1: (Z.to_nat (i + Zlength key) < length (HMAC_SHA256.mkKey key))%nat).
            rewrite mkKey_length; unfold SHA256.BlockSize.
-           destruct H1. 
+           destruct XX as [XX YY]. 
            apply (Z2Nat.inj_lt (i+ Zlength key) 64). omega. omega. omega.
          rewrite nth_map' with (d':=Int.zero).
          rewrite nth_map' with (d':=Z0). f_equal.
@@ -702,9 +754,14 @@ forward_if PostKeyNull.
      rewrite data_at__isptr. normalize.
      apply isptrD in H4. destruct H4 as [pb [pofs PAD]].
      apply exp_right with (x:=Vptr pb pofs).
-   entailer.
-     apply exp_right with (x:=1). entailer. cancel.
-     if_tac; try omega. rewrite PAD; cancel.
+   entailer. 
+     apply exp_right with (x:=1). entailer.
+     apply isptrD in H5. destruct H5 as [ckb [ckofs CK]].
+     apply exp_right with (x:=Vptr ckb ckofs).
+     entailer. cancel.
+     if_tac; try omega. rewrite PAD, CK; cancel.
+     apply exp_right with (x:= Zlength key).
+     entailer. apply prop_right. unfold has_lengthK; clear H. split; trivial. split; trivial.
   }
   { (*key == NULL*)
      forward. normalize. rewrite HeqPostKeyNull. clear  HeqPostKeyNull. normalize.
@@ -720,8 +777,11 @@ forward_if PostKeyNull.
         apply exp_right with (x:=cofs).
         apply exp_right with (x:=Vptr pb pofs).
         apply exp_right with (x:=0). entailer. rewrite PAD. cancel.
+        apply isptrD in H2. destruct H2 as [ckb [ckofs CK]].
+        apply exp_right with (x:=Vptr ckb ckofs). entailer. cancel. 
         if_tac; try omega.
-          apply exp_right with (x:=r). apply exp_right with (x:=v). entailer.
+          apply exp_right with (x:=r). rewrite CK; cancel. 
+          apply exp_right with (x:=v). entailer.
      inversion H0.
   }
   { (*side condition of forward_if key != NULL*)
