sha/HMAC_lemmas.v
@@ -62,33 +62,33 @@ Proof. intros n.
 Qed. 
 
 Lemma first64_sixtyfour {A} (a:A): 
-      firstn 64 (sixtyfour a) = sixtyfour a.
+      firstn 64 (HMAC_SHA256.sixtyfour a) = HMAC_SHA256.sixtyfour a.
 Proof. apply firstn_precise. simpl. reflexivity. Qed. 
 
-Lemma length_Nlist {A} (i:A): forall n, length (Nlist i n) = n.
+Lemma length_Nlist {A} (i:A): forall n, length (HMAC_SHA256.Nlist i n) = n.
 Proof. induction n; simpl; auto. Qed.
 
-Lemma length_SF {A} (x:A): length (sixtyfour x) = 64%nat.
-Proof. unfold sixtyfour. rewrite length_Nlist; trivial. Qed.
+Lemma length_SF {A} (x:A): length (HMAC_SHA256.sixtyfour x) = 64%nat.
+Proof. unfold HMAC_SHA256.sixtyfour. rewrite length_Nlist; trivial. Qed.
 
 Lemma str_to_Z_length: forall k, 
       String.length k = length (str_to_Z k).
 Proof. intros. induction k; simpl; auto. Qed.
   
-Lemma Zlength_mkArgZ k pad: Zlength (HMAC_FUN.mkArgZ k pad) = Z.of_nat (min (length k) 64).
+Lemma Zlength_mkArgZ k pad: Zlength (HMAC_SHA256.mkArgZ k pad) = Z.of_nat (min (length k) 64).
 Proof. intros. repeat rewrite Zlength_correct.
-   unfold HMAC_FUN.mkArgZ, HMAC_FUN.mkArg, sixtyfour.
+   unfold HMAC_SHA256.mkArgZ, HMAC_SHA256.mkArg, HMAC_SHA256.sixtyfour.
    repeat rewrite map_length. 
    rewrite combine_length, length_Nlist. trivial.
 Qed. 
 
-Lemma In_Nlist {A:Type}: forall (n:A) l x, In x (Nlist n l) -> x=n.
+Lemma In_Nlist {A:Type}: forall (n:A) l x, In x (HMAC_SHA256.Nlist n l) -> x=n.
 Proof. intros n l.
   induction l; simpl; intros. contradiction.
   destruct H; eauto.
 Qed.
-Lemma zeropad_isbyteZ: forall l, Forall isbyteZ l -> Forall isbyteZ (HMAC_FUN.zeroPad l).
-Proof. unfold isbyteZ, HMAC_FUN.zeroPad; intros.
+Lemma zeropad_isbyteZ: forall l, Forall isbyteZ l -> Forall isbyteZ (HMAC_SHA256.zeroPad l).
+Proof. unfold isbyteZ, HMAC_SHA256.zeroPad; intros.
   rewrite Forall_forall in *. intros.
   apply in_app_or in H0.
   destruct H0. apply (H _ H0).
@@ -172,7 +172,7 @@ apply H0.
 Qed.
 
 Lemma nth_Nlist {A}: forall (a d:A) k i (Hik: (i <k)%nat),
-      nth i (Nlist a k) d = a.
+      nth i (HMAC_SHA256.Nlist a k) d = a.
 Proof. intros a d k.
   induction k; simpl. 
     intros. omega.
@@ -181,7 +181,7 @@ Proof. intros a d k.
 Qed. 
 
 Lemma map_Nlist: forall {A B} a (f:A -> B) n,
-                 map f (Nlist a n) = Nlist (f a) n.
+                 map f (HMAC_SHA256.Nlist a n) = HMAC_SHA256.Nlist (f a) n.
 Proof. intros. induction n; simpl; trivial. rewrite IHn. trivial. Qed.
 
 Lemma minus_lt_compat_r: forall n m p : nat,
@@ -215,8 +215,8 @@ Proof.
 Qed.
 
 Lemma nth_zeropad_left {d d'}: forall l i (I: 0<= i < Zlength l),
-      nth (Z.to_nat i) (HMAC_FUN.zeroPad l) d = nth (Z.to_nat i) l d'.
-Proof. unfold HMAC_FUN.zeroPad. intros.
+      nth (Z.to_nat i) (HMAC_SHA256.zeroPad l) d = nth (Z.to_nat i) l d'.
+Proof. unfold HMAC_SHA256.zeroPad. intros.
   destruct I.
   apply Z2Nat.inj_lt in H0; try omega.
   rewrite Zlength_correct, Nat2Z.id in H0.
@@ -226,14 +226,14 @@ Qed.
 
 Lemma mkKey_left {d d'}: forall l (L: false = (Zlength l >? 64)) 
         i (I: 0<= i < Zlength l),
-      nth (Z.to_nat i) (HMAC_FUN.mkKey l) d = nth (Z.to_nat i) l d'.
+      nth (Z.to_nat i) (HMAC_SHA256.mkKey l) d = nth (Z.to_nat i) l d'.
 Proof.
-  unfold HMAC_FUN.mkKey. intros. simpl. rewrite <- L.
+  unfold HMAC_SHA256.mkKey. intros. simpl. rewrite <- L.
   apply nth_zeropad_left; trivial.
 Qed.
 Lemma nth_zeropad_right {d}: forall l i (I: Zlength l <= i < 64),
-      nth (Z.to_nat i) (HMAC_FUN.zeroPad l) d = Z0.
-Proof. unfold HMAC_FUN.zeroPad. intros.
+      nth (Z.to_nat i) (HMAC_SHA256.zeroPad l) d = Z0.
+Proof. unfold HMAC_SHA256.zeroPad. intros.
   rewrite app_nth2. rewrite nth_Nlist. trivial.
   apply minus_lt_compat_r. destruct I. apply Z2Nat.inj_lt in H0. apply H0.
   specialize (initial_world.zlength_nonneg _ l). omega.
@@ -247,9 +247,9 @@ Proof. unfold HMAC_FUN.zeroPad. intros.
 Qed.
 Lemma mkKey_right {d}: forall l (L: false = (Zlength l >? 64)) 
         i (I: Zlength l <= i < 64),
-      nth (Z.to_nat i) (HMAC_FUN.mkKey l) d = Z0.
+      nth (Z.to_nat i) (HMAC_SHA256.mkKey l) d = Z0.
 Proof.
-  unfold HMAC_FUN.mkKey. intros. simpl. rewrite <- L.
+  unfold HMAC_SHA256.mkKey. intros. simpl. rewrite <- L.
   apply nth_zeropad_right; trivial.
 Qed.
 
@@ -387,34 +387,34 @@ rewrite (split_offset_array_at_ _ _ _ p).
  assumption. simpl; omega. reflexivity. apply isptr_offset_val'; trivial.
 Qed.
 
-Lemma zeroPad_BlockSize: forall k, (length k <= SHA256_BlockSize)%nat ->
-  length (HMAC_FUN.zeroPad k) = SHA256_BlockSize%nat.
-Proof. unfold HMAC_FUN.zeroPad. intros. rewrite app_length, length_Nlist. omega. 
+Lemma zeroPad_BlockSize: forall k, (length k <= SHA256.BlockSize)%nat ->
+  length (HMAC_SHA256.zeroPad k) = SHA256.BlockSize%nat.
+Proof. unfold HMAC_SHA256.zeroPad. intros. rewrite app_length, length_Nlist. omega. 
 Qed. 
 
 Lemma length_SHA256': forall l, 
-  length (functional_prog.SHA_256' l) = Z.to_nat SHA256_DIGEST_LENGTH.
+  length (functional_prog.SHA_256' l) = SHA256.DigestLength.
 Proof. intros. unfold functional_prog.SHA_256'. simpl.
   rewrite length_intlist_to_Zlist, functional_prog.length_process_msg. reflexivity.
 Qed.
  
-Lemma mkKey_length l: length (HMAC_FUN.mkKey l) = SHA256_BlockSize.
-Proof. intros. unfold HMAC_FUN.mkKey.
-  remember (Zlength l >? Z.of_nat SHA256_BlockSize) as z. 
+Lemma mkKey_length l: length (HMAC_SHA256.mkKey l) = SHA256.BlockSize.
+Proof. intros. unfold HMAC_SHA256.mkKey.
+  remember (Zlength l >? Z.of_nat SHA256.BlockSize) as z. 
   destruct z. apply zeroPad_BlockSize.
     rewrite length_SHA256'.  
     apply Nat2Z.inj_le. simpl. omega. 
   apply zeroPad_BlockSize.
     rewrite Zlength_correct in Heqz. 
     apply Nat2Z.inj_le. 
-    specialize (Zgt_cases (Z.of_nat (Datatypes.length l)) (Z.of_nat SHA256_BlockSize)). rewrite <- Heqz. trivial.
+    specialize (Zgt_cases (Z.of_nat (Datatypes.length l)) (Z.of_nat SHA256.BlockSize)). rewrite <- Heqz. trivial.
 Qed.
 
-Lemma mkKey_atBlockSize s: length s = SHA256_BlockSize%nat ->
-      HMAC_FUN.mkKey s = s.
-Proof. unfold HMAC_FUN.mkKey. rewrite Zlength_correct.
+Lemma mkKey_atBlockSize s: length s = SHA256.BlockSize%nat ->
+      HMAC_SHA256.mkKey s = s.
+Proof. unfold HMAC_SHA256.mkKey. rewrite Zlength_correct.
   intros. rewrite H.
-  simpl. unfold HMAC_FUN.zeroPad. rewrite H. simpl.
+  simpl. unfold HMAC_SHA256.zeroPad. rewrite H. simpl.
   apply app_nil_r.  
 Qed.
 
@@ -449,12 +449,12 @@ Proof. intros.
        apply (initial_world.zlength_nonneg _ l).
 Qed.
 
-Lemma HMAC_length d k: length (HMAC_FUN.HMAC d k) = 32%nat.
+Lemma HMAC_length d k: length (HMAC_SHA256.HMAC d k) = 32%nat.
 Proof.
-  unfold HMAC_FUN.HMAC, HMAC_FUN.OUTER.
+  unfold HMAC_SHA256.HMAC, HMAC_SHA256.OUTER.
   apply length_SHA256'.
 Qed.
-Lemma HMAC_Zlength d k: Zlength (HMAC_FUN.HMAC d k) = 32.
+Lemma HMAC_Zlength d k: Zlength (HMAC_SHA256.HMAC d k) = 32.
 Proof.
   rewrite Zlength_correct, HMAC_length. reflexivity.
 Qed.
