sha/verif_hmacADT_init.v
@@ -7,12 +7,12 @@ Local Open Scope logic.
 Require Import sha.spec_sha.
 Require Import sha_lemmas.
 Require Import sha.HMAC_functional_prog.
-Require Import sha.spec_hmac.
+Require Import sha.spec_hmacADT.
 Require Import HMAC_lemmas.
 
-Require Import sha.hmac091c.
+Require Import sha.hmac_NK.
 
-Require Import sha.verif_hmac_init_part1.
+Require Import sha.verif_hmacADT_init_part1.
 
 Lemma ZnthV_map_Vint_is_int_I8: forall l (i : Z) ,
        0 <= i < Zlength l -> 
@@ -101,10 +101,8 @@ Proof. intros. unfold cVint, ZnthV, upd. if_tac. omega. simpl.
                apply Byte.bits_above. apply H1.
 Qed.
 
-Definition postResetHMS key (iS oS: s256state): hmacstate :=
-  (emptySha, (iS, (oS, 
-   (if zlt 64 (Zlength key) then Vint (Int.repr 32) else Vint (Int.repr (Zlength key)), 
-   map Vint (map Int.repr (HMAC_SHA256.mkKey key)))))).
+Definition postResetHMS (iS oS: s256state): hmacstate :=
+  (emptySha, (iS, oS)).
 
 Lemma body_hmac_init: semax_body HmacVarSpecs HmacFunSpecs 
        f_HMAC_Init HMAC_Init_spec.
@@ -114,27 +112,8 @@ name ctx' _ctx.
 name key' _key.
 name len' _len.
 simpl_stackframe_of.
-destruct H as [KL1 [KL2 KL3]]. normalize.
-(*
-eapply semax_pre with (P':=PROP  (isptr k /\ Forall isbyteZ key /\ isptr c)
-   LOCAL  (`(eq c) (eval_id _ctx); `(eq k) (eval_id _key);
-   `(eq (Vint (Int.repr l))) (eval_id _len);
-   `(eq KV) (eval_var sha._K256 (tarray tuint 64)))
-   SEP 
-   ((EX pad:_, 
-            local (`(eq pad) (eval_var _pad (tarray tuchar 64))) && 
-            `(data_at_ Tsh (tarray tuchar 64) pad));
-   `(data_at_ Tsh t_struct_hmac_ctx_st c); `(data_block Tsh key k);
-   `(K_vector KV))).
-  entailer. apply exp_right with (x:=eval_var _pad (tarray tuchar 64) rho). 
-  entailer. 
-normalize. intros pad. normalize. 
-apply isptrD in H. destruct H as [kb [kofs isptr_k]]; rewrite isptr_k in *.
-apply isptrD in H1. destruct H1 as [cb [cofs isptr_c]]; rewrite isptr_c in *.
-rename H0 into isbyte_key.
-*)
-(*Sset _reset (Econst_int (Int.repr 0) tint)*)
-forward.
+(*destruct H as [KL1 [KL2 KL3]].*) normalize.
+forward. 
 
 unfold data_block. normalize. 
 
@@ -144,40 +123,40 @@ apply seq_assoc.
 remember (EX  cb : block,
                  (EX  cofs : int,
                   (EX  pad : val,
-                   (EX  r : Z,
-                    PROP  (c = Vptr cb cofs/\ (r=0 \/ r=1))
+                   (EX  r : Z, EX ctxkey:val,
+                    PROP  (c = Vptr cb cofs /\ (r=0 \/ r=1))
                     LOCAL  (`(eq (Vint (Int.repr r))) (eval_id _reset);
                     `(eq pad) (eval_var _pad (tarray tuchar 64));
                     `(eq c) (eval_id _ctx); `(eq k) (eval_id _key);
-                    `(eq (Vint (Int.repr l))) (eval_id _len);
+                    `(eq l) (eval_id _len);
+                    `(eq ctxkey) (eval_var _ctx_key (tarray tuchar 64));
                     `(eq KV) (eval_var sha._K256 (tarray tuint 64)))
                     SEP  (`(data_at_ Tsh (tarray tuchar 64) pad);
-                    `(initPostKeyNullConditional r c k h1 key);
+                    `(initPostKeyNullConditional l r c k h1 key ctxkey);
                     `(K_vector KV)))))) as PostKeyNull. 
 forward_seq. instantiate (1:= PostKeyNull). (*eapply semax_seq.*)
-{ assert (DD: Delta = initialized _reset 
-               (func_tycontext f_HMAC_Init HmacVarSpecs HmacFunSpecs)) by reflexivity.
-  rewrite DD; clear DD.
-  eapply hmac_init_part1; eassumption.
+{  assert (DD: Delta= initialized _reset Delta) by reflexivity.
+   rewrite DD.
+   eapply hmac_init_part1; eassumption. 
 }
 subst PostKeyNull. normalize.
 apply extract_exists_pre; intros cb. 
 apply extract_exists_pre; intros cofs. 
 apply extract_exists_pre; intros pad. 
 apply extract_exists_pre; intros r.
+apply extract_exists_pre; intros ctxkey.
 normalize. rename H into HC; rewrite HC. rename H0 into R.
 
 (*isolate branch if (reset) *)
 apply seq_assoc.
-
-Definition initPostResetConditional r (c:val) (k: val) h key iS oS: mpred:=
+Definition initPostResetConditional l r (c:val) (k: val) h key iS oS: mpred:=
   match k with
     Vint z => if Int.eq z Int.zero
               then if zeq r Z0 then hmacstate_PreInitNull key h c else FF
               else FF
   | Vptr b ofs => if zeq r 0 then FF
-                  else !!(Forall isbyteZ key) &&
-                       ((data_at Tsh t_struct_hmac_ctx_st (postResetHMS key iS oS) c) *
+                  else EX ll:_, !!(Forall isbyteZ key/\ has_lengthK ll key /\ l = Vint(Int.repr ll)) &&
+                       ((data_at Tsh t_struct_hmac_ctx_st (postResetHMS iS oS) c) *
                         (array_at tuchar Tsh (tuchars (map Int.repr key)) 0 (Zlength key) (Vptr b ofs)))
   | _ => FF
   end.
@@ -188,13 +167,14 @@ remember (EX iSA:_, EX iS:_, EX oSA:_, EX oS:_,
                  LOCAL  (
                  `(eq pad) (eval_var _pad (tarray tuchar 64));
                  `(eq (Vptr cb cofs)) (eval_id _ctx);
+                 `(eq ctxkey) (eval_var _ctx_key (tarray tuchar 64));
                  `(eq k) (eval_id _key);
-                 `(eq (Vint (Int.repr l))) (eval_id _len);
+                 `(eq l) (eval_id _len);
                  `(eq KV) (eval_var sha._K256 (tarray tuint 64)))
 
                  SEP  (
-                 `(array_at_ tuchar Tsh 0 64 pad); 
-                 `(initPostResetConditional r c k h1 key iS oS); `(K_vector KV)))
+                 `(array_at_ tuchar Tsh 0 64 pad); `(data_at_ Tsh (tarray tuchar 64) ctxkey);
+                 `(initPostResetConditional l r c k h1 key iS oS); `(K_vector KV)))
   as PostResetBranch.
 (*forward_seq. instantiate (1:= PostResetBranch).*)
 eapply semax_seq. instantiate (1:=PostResetBranch).
@@ -216,34 +196,38 @@ eapply semax_seq. instantiate (1:=PostResetBranch).
     unfold data_at_, tuchars, tarray.
     erewrite data_at_array_at; try reflexivity. 2: omega.
     rewrite array_at_isptr. normalize. apply isptrD in H. destruct H as [pb [pofs Hpad]]. subst pad.
-    apply semax_pre with (P':=PROP  (r<>0 /\ Forall isbyteZ key)
+    apply semax_pre with (P':=EX ll:_,
+         PROP  (r<>0 /\ Forall isbyteZ key/\ has_lengthK ll key /\ l = Vint(Int.repr ll))
          LOCAL  (tc_environ Delta;
             `(eq (Vint (Int.repr r))) (eval_id _reset);
             `(eq (Vptr pb pofs)) (eval_var _pad (Tarray tuchar 64 noattr));
             `(eq (Vptr cb cofs)) (eval_id _ctx); `(eq k) (eval_id _key);
-            `(eq (Vint (Int.repr l))) (eval_id _len);
+            `(eq l) (eval_id _len);
+            `(eq ctxkey) (eval_var _ctx_key (Tarray tuchar 64 noattr));
             `(eq KV) (eval_var sha._K256 (Tarray tuint 64 noattr)))
          SEP  (`(K_vector KV);
                `(array_at tuchar Tsh (ZnthV tuchar (default_val (Tarray tuchar 64 noattr)))
                    0 64 (Vptr pb pofs));
-               `(data_at Tsh t_struct_hmac_ctx_st (keyedHMS key) (Vptr cb cofs));
+               `(data_at Tsh t_struct_hmac_ctx_st keyedHMS (Vptr cb cofs));
+               `(data_at Tsh (tarray tuchar 64) (map Vint (map Int.repr (HMAC_SHA256.mkKey key)))
+                  ctxkey);
                `(array_at tuchar Tsh (tuchars (map Int.repr key)) 0 (Zlength key) k))).
     { clear HeqPostResetBranch PostResetBranch.
       unfold initPostKeyNullConditional. entailer.
       destruct key'; try contradiction.
       (*integer, ie key==NULL*)
-          simpl in TC0. subst i. simpl. if_tac. subst r. inversion H0.
-          apply andp_right. entailer. entailer.
+          simpl in TC0. subst i. simpl. if_tac. subst r. inversion H0. normalize.
       (*key == Vptr*)
-       if_tac. subst r.
-          unfold typed_true in H0. simpl in H0. inversion H0.
-          entailer. cancel.
+       if_tac. normalize. entailer. apply exp_right with (x:=ll); entailer. cancel.
     }
+    apply extract_exists_pre. intros ll; normalize. subst l; rename ll into l.
+    rename H0 into isbyte_key. rename H1 into KL.
     rewrite (array_at_isptr _ _ _ _ _ k). normalize.
     destruct R; subst r. omega. clear H. 
-    rename H0 into isbyte_key.
-    apply isptrD in H1; destruct H1 as [kb [kofs HK]]; rewrite HK in *.
-    
+    apply isptrD in H0; destruct H0 as [kb [kofs HK]]; rewrite HK in *.
+    rewrite data_at_isptr with (p:=ctxkey). normalize.
+    apply isptrD in H; destruct H as [ckb [ckofs HCK]]; rewrite HCK in *.
+
     forward_seq. 
     instantiate (1:= 
       (PROP  ()
@@ -252,10 +236,13 @@ eapply semax_seq. instantiate (1:=PostResetBranch).
         `(eq (Vptr pb pofs)) (eval_var _pad (Tarray tuchar 64 noattr));
         `(eq (Vptr cb cofs)) (eval_id _ctx); `(eq k) (eval_id _key);
         `(eq (Vint (Int.repr l))) (eval_id _len);
+        `(eq ctxkey) (eval_var _ctx_key (Tarray tuchar 64 noattr));
         `(eq KV) (eval_var sha._K256 (tarray tuint 64)))
        SEP 
         (`(array_at tuchar Tsh IPADcont 0 64 (Vptr pb pofs));
-         `(data_at Tsh t_struct_hmac_ctx_st (keyedHMS key) (Vptr cb cofs));
+         `(data_at Tsh t_struct_hmac_ctx_st keyedHMS (Vptr cb cofs));
+         `(data_at Tsh (tarray tuchar 64)
+              (map Vint (map Int.repr (HMAC_SHA256.mkKey key))) (Vptr ckb ckofs));
          `(array_at tuchar Tsh (tuchars (map Int.repr key)) 0 (Zlength key) (Vptr kb kofs));
         `(K_vector KV)))).
     { (*ipad loop*)
@@ -265,12 +252,15 @@ eapply semax_seq. instantiate (1:=PostResetBranch).
                  `(eq (Vptr pb pofs)) (eval_var _pad (tarray tuchar 64));
                  `(eq (Vptr cb cofs)) (eval_id _ctx);
                  `(eq (Vptr kb kofs)) (eval_id _key);
+                 `(eq ctxkey) (eval_var _ctx_key (Tarray tuchar 64 noattr));
                  `(eq (Vint (Int.repr l))) (eval_id _len);
                  `(eq KV) (eval_var sha._K256 (tarray tuint 64)))
          SEP  (
           `(array_at tuchar Tsh IPADcont 0 i (Vptr pb pofs));
           `(array_at tuchar Tsh DEFAULTcont i 64 (Vptr pb pofs));
-          `(data_at Tsh t_struct_hmac_ctx_st (keyedHMS key) (Vptr cb cofs));
+          `(data_at Tsh t_struct_hmac_ctx_st keyedHMS (Vptr cb cofs));
+         `(data_at Tsh (tarray tuchar 64)
+              (map Vint (map Int.repr (HMAC_SHA256.mkKey key))) (Vptr ckb ckofs));
           `(array_at tuchar Tsh (ZnthV tuchar (map Vint (map Int.repr key))) 0
                (Zlength key) (Vptr kb kofs)); `(K_vector KV)))).
       { (*precondition implies "invariant"*) 
@@ -280,11 +270,12 @@ eapply semax_seq. instantiate (1:=PostResetBranch).
       { unfold normal_ret_assert. simpl. intros rho. 
         rewrite array_at_emp. entailer.
       }
-      { unfold_data_at 1%nat. normalize.
+      { rename H into I. 
+        (*unfold_data_at 1%nat. normalize.
         rewrite (field_at_data_at Tsh t_struct_hmac_ctx_st [_key]); try reflexivity.
-        normalize. rename H into I. rename H0 into SCc. rename H1 into ACc.
+        normalize. rename H0 into SCc. rename H1 into ACc.
         rewrite at_offset'_eq.
-        2: simpl; rewrite Int.add_zero; reflexivity.
+        2: simpl; rewrite Int.add_zero; reflexivity.*)
         eapply semax_pre0; [ apply now_later | ].
         eapply semax_post_flipped'.
         { subst PostResetBranch.
@@ -295,92 +286,59 @@ eapply semax_seq. instantiate (1:=PostResetBranch).
           assert (Hres: ZnthV tuchar (map Vint (map Int.repr
                    (HMAC_SHA256.mkArgZ (map Byte.repr (HMAC_SHA256.mkKey key)) HMAC_SHA256.Ipad))) i
               = Vint (Int.zero_ext 8 (Int.xor (Int.repr 54) N))). 
-          { clear - HN I isbyte_key. apply xor_pad_result; assumption. }
-          eapply NEWsemax_loadstore_array
-          with (P:= nil)
-          (Q:= [`(eq (Vint (Int.repr i))) (eval_id _i);
-            `(eq (Vint (Int.repr 64))) (eval_expr (Econst_int (Int.repr 64) tint));
-            `(eq (Vint (Int.repr 1))) (eval_id _reset);
-            `(eq (Vptr pb pofs)) (eval_var _pad (tarray tuchar 64));
-            `(eq (Vptr cb cofs)) (eval_id _ctx);
-            `(eq (Vptr kb kofs)) (eval_id _key);
-            `(eq (Vint (Int.repr l))) (eval_id _len);
-            `(eq KV) (eval_var sha._K256 (tarray tuint 64))])
-          (R:= [`(field_at Tsh t_struct_hmac_ctx_st [_key_length]
-               (if zlt 64 (Zlength key)
-                then Vint (Int.repr 32)
-                else Vint (Int.repr (Zlength key))) (Vptr cb cofs));
-            `(data_at Tsh (nested_field_type2 t_struct_hmac_ctx_st [_key])
-                (map Vint (map Int.repr (HMAC_SHA256.mkKey key)))
-               (offset_val
-                 (Int.repr (nested_field_offset2 t_struct_hmac_ctx_st [_key]))
-                 (Vptr cb cofs)));
-            `(field_at Tsh t_struct_hmac_ctx_st [_o_ctx] emptySha (Vptr cb cofs));
-            `(field_at Tsh t_struct_hmac_ctx_st [_i_ctx] emptySha (Vptr cb cofs));
-            `(field_at Tsh t_struct_hmac_ctx_st [_md_ctx] emptySha (Vptr cb cofs));
-            `(array_at tuchar Tsh IPADcont 0 i (Vptr pb pofs));
-            `(array_at tuchar Tsh DEFAULTcont i 64 (Vptr pb pofs));
-            `(array_at tuchar Tsh (ZnthV tuchar (map Vint (map Int.repr key))) 0
-                (Zlength key) (Vptr kb kofs)); `(K_vector KV)])
-          (n:=6%nat)
-          (v2:=(ZnthV tuchar (map Vint(map Int.repr (HMAC_SHA256.mkArgZ (map Byte.repr (HMAC_SHA256.mkKey key)) HMAC_SHA256.Ipad))) i)).
-          simpl; try reflexivity.
-          simpl; try reflexivity.
-          simpl; try reflexivity.
-          simpl; try reflexivity.
-          simpl; try reflexivity.
-          Focus 2. simpl. unfold value, nested_field_type2, t_struct_hmac_ctx_st; simpl.
-            reflexivity.
-          2: trivial.     
-          instantiate (1:=i). unfold nested_field_offset2, _struct_SHA256state_st; simpl.
-          intros rho. normalize.
-           apply andp_right. apply andp_right; rel_expr.
-           rewrite Hres.
-           erewrite (data_at_type_changable Tsh _ (tarray tuchar 64)); try reflexivity.
-           unfold tarray. 
-           erewrite data_at_array_at; try reflexivity.
-           erewrite (split3_array_at' i); try reflexivity. 2: trivial. 2: omega.
-           {  rel_expr.  instantiate (1:=cofs). instantiate (1:=cb).
-              rel_expr.
-                  admit. (*relexpr*)
-             unfold nested_field_offset2, _struct_SHA256state_st; simpl.
-              instantiate (2:=Tsh). unfold add_ptr_int. simpl.
-              instantiate (1:=(ZnthV tuchar (map Vint (map Int.repr (HMAC_SHA256.mkKey key))) i)).
+          { clear - HN I isbyte_key. apply xor_pad_result; try assumption. }
+            unfold tarray. 
+            erewrite data_at_array_at with (v:= map Vint (map Int.repr (HMAC_SHA256.mkKey key))); try reflexivity.
+              2: omega. 
+            eapply NEWsemax_loadstore_array with 
+              (n:=1%nat)
+              (v2:=(ZnthV tuchar (map Vint(map Int.repr (HMAC_SHA256.mkArgZ (map Byte.repr (HMAC_SHA256.mkKey key)) HMAC_SHA256.Ipad))) i)).
+             simpl; try reflexivity.
+             simpl; try reflexivity.
+             simpl; try reflexivity.
+             simpl; try reflexivity.
+             simpl; try reflexivity.
+             { instantiate (1:=i). instantiate (1:=Vptr pb pofs).
+               entailer. normalize. 
+               apply andp_right. apply andp_right; rel_expr. 
+               rewrite Hres. 
+               erewrite (split3_array_at' i _ _ _ 0 64); try reflexivity. 2: trivial.
+               { rel_expr. 
+                 unfold ZnthV in *. if_tac. omega. simpl; rewrite HN. discriminate.
+                 simpl; intros.
+                 unfold ZnthV in *. if_tac. omega. simpl; rewrite HN. reflexivity.
+                 reflexivity.
+               } 
+             } 
+             simpl. reflexivity.
+             trivial.
+             { unfold HMAC_SHA256.mkArgZ. simpl. apply ZnthV_map_Vint_is_int_I8.
+               unfold HMAC_SHA256.mkArgZ in ZLI. rewrite Zlength_correct, map_length in ZLI. 
+               rewrite Zlength_correct, ZLI. omega.
+             }
+             red; omega.   
+          }
+          { entailer. cancel.
+            rewrite (split_array_at (i+1) tuchar Tsh _ i 64); try omega. cancel.
+            unfold tarray. erewrite data_at_array_at; try reflexivity.
+              2: omega.
+            cancel. 
+            apply sepcon_derives.
+              rewrite (split_array_at i tuchar Tsh _ 0 (i+1)); try omega.
               cancel.
-             unfold ZnthV in *. if_tac. omega. simpl; rewrite HN. discriminate.
-             simpl; intros.
-                unfold ZnthV in *. if_tac. omega. simpl; rewrite HN. reflexivity.
-             reflexivity.
-           }
-           { unfold HMAC_SHA256.mkArgZ. simpl. apply ZnthV_map_Vint_is_int_I8.
-             unfold HMAC_SHA256.mkArgZ in ZLI. rewrite Zlength_correct, map_length in ZLI. 
-             rewrite Zlength_correct, ZLI. omega.
-           }
-           red; omega.
-        }
-        { entailer. cancel.
-          rewrite (split_array_at (i+1) tuchar Tsh _ i 64); try omega. cancel.
-          unfold_data_at 2%nat. cancel.
-          rewrite (field_at_data_at Tsh t_struct_hmac_ctx_st [_key]); try reflexivity.
-          entailer.
-          rewrite at_offset'_eq.
-          2: simpl; rewrite Int.add_zero; reflexivity. unfold offset_val. cancel.
-          apply sepcon_derives.
-            rewrite (split_array_at i tuchar Tsh _ 0 (i+1)); try omega.
-            cancel.
+              apply array_lemmas.array_at_ext'.
+              unfold cVint, ZnthV; simpl; intros.
+              assert (i0=i). omega. subst i0. simpl.
+              destruct (zlt i 0). omega. simpl. rewrite upd_eq.
+              destruct (nth_mapVintZ i 
+               (HMAC_SHA256.mkArgZ (map Byte.repr (HMAC_SHA256.mkKey key)) HMAC_SHA256.Ipad)) as [n Hn].
+              rewrite ZLI; assumption.
+              rewrite Hn. unfold HMAC_SHA256.mkArgZ in Hn; rewrite Hn. trivial.
             apply array_lemmas.array_at_ext'.
-            unfold cVint, ZnthV; simpl; intros.
-            assert (i0=i). omega. subst i0. simpl.
-            destruct (zlt i 0). omega. simpl. rewrite upd_eq.
-            destruct (nth_mapVintZ i 
-             (HMAC_SHA256.mkArgZ (map Byte.repr (HMAC_SHA256.mkKey key)) HMAC_SHA256.Ipad)) as [n Hn].
-             rewrite ZLI; assumption.
-            rewrite Hn. unfold HMAC_SHA256.mkArgZ in Hn; rewrite Hn. trivial.
-          apply array_lemmas.array_at_ext'.
-            unfold cVint, ZnthV; simpl; intros. rewrite upd_neq; trivial. omega.
-        } 
+              unfold cVint, ZnthV; simpl; intros. rewrite upd_neq; trivial. omega.
+          } 
+        }
       }
-    }
 
     (*continuation after ipad-loop*)   
     unfold_data_at 1%nat. normalize.
@@ -388,7 +346,7 @@ eapply semax_seq. instantiate (1:=PostResetBranch).
     rewrite at_offset'_eq.
     2: simpl; rewrite Int.add_zero; reflexivity.
     eapply semax_seq'.
-    frame_SEP 3.
+    frame_SEP 0.
     forward_call (Vptr cb (Int.add cofs (Int.repr 108))).
     { assert (FR: Frame = nil).
         subst Frame. reflexivity.
@@ -398,7 +356,7 @@ eapply semax_seq. instantiate (1:=PostResetBranch).
     after_call. simpl. normalize. 
 
     eapply semax_seq'.
-    frame_SEP 0 5 7.
+    frame_SEP 0 3 6.
     remember (init_s256abs, 
             HMAC_SHA256.mkArgZ (map Byte.repr (HMAC_SHA256.mkKey key)) HMAC_SHA256.Ipad,
             Vptr cb (Int.add cofs (Int.repr 108)),
@@ -426,15 +384,16 @@ eapply semax_seq. instantiate (1:=PostResetBranch).
 
     simpl.
     apply semax_pre with (P':=EX x : s256abs,
-     (PROP  ()
-     LOCAL  (tc_environ Delta; tc_environ Delta;
-       `(eq (Vint (Int.repr 1))) (eval_id _reset);
-       `(eq (Vptr pb pofs)) (eval_var _pad (Tarray tuchar 64 noattr));
-       `(eq (Vptr cb cofs)) (eval_id _ctx); `(eq (Vptr kb kofs)) (eval_id _key);
-       `(eq (Vint (Int.repr l))) (eval_id _len);
-       `(eq KV) (eval_var sha._K256 (tarray tuint 64)))
-     SEP 
-      (`(fun a : environ =>
+  (PROP  ()
+   LOCAL  (tc_environ Delta; tc_environ Delta;
+   `(eq (Vint (Int.repr 1))) (eval_id _reset);
+   `(eq (Vptr pb pofs)) (eval_var _pad (Tarray tuchar 64 noattr));
+   `(eq (Vptr cb cofs)) (eval_id _ctx); `(eq k) (eval_id _key);
+   `(eq (Vint (Int.repr l))) (eval_id _len);
+   `(eq ctxkey) (eval_var _ctx_key (Tarray tuchar 64 noattr));
+   `(eq KV) (eval_var sha._K256 (tarray tuint 64)))
+   SEP 
+   (`(fun a : environ =>
       (PROP 
        (update_abs
           (HMAC_SHA256.mkArgZ (map Byte.repr (HMAC_SHA256.mkKey key)) HMAC_SHA256.Ipad)
@@ -445,16 +404,12 @@ eapply semax_seq. instantiate (1:=PostResetBranch).
        `(data_block Tsh
            (HMAC_SHA256.mkArgZ (map Byte.repr (HMAC_SHA256.mkKey key)) HMAC_SHA256.Ipad)
            (Vptr pb pofs)))) a) globals_only;
-      `(field_at Tsh t_struct_hmac_ctx_st [_key_length]
-          (if zlt 64 (Zlength key)
-           then Vint (Int.repr 32)
-           else Vint (Int.repr (Zlength key))) (Vptr cb cofs));
-      `(field_at Tsh t_struct_hmac_ctx_st [_key]
-          (map Vint (map Int.repr (HMAC_SHA256.mkKey key))) (Vptr cb cofs));
-      `(field_at Tsh t_struct_hmac_ctx_st [_o_ctx] emptySha (Vptr cb cofs));
-      `(field_at Tsh t_struct_hmac_ctx_st [_md_ctx] emptySha (Vptr cb cofs));
-      `(array_at tuchar Tsh (tuchars (map Int.repr key)) 0 (Zlength key)
-         (Vptr kb kofs))))).
+   `(field_at Tsh t_struct_hmac_ctx_st [_o_ctx] emptySha (Vptr cb cofs));
+   `(field_at Tsh t_struct_hmac_ctx_st [_md_ctx] emptySha (Vptr cb cofs));
+   `(data_at Tsh (tarray tuchar 64)
+       (map Vint (map Int.repr (HMAC_SHA256.mkKey key))) (Vptr ckb ckofs));
+   `(array_at tuchar Tsh (tuchars (map Int.repr key)) 0 (Zlength key)
+       (Vptr kb kofs))))).
     entailer. rename x into a. eapply exp_right with (x:=a). entailer.
     apply extract_exists_pre. intros ipadSHAabs.
     rename H into SCc.
@@ -474,23 +429,20 @@ eapply semax_seq. instantiate (1:=PostResetBranch).
    `(eq (Vptr pb pofs)) (eval_var _pad (Tarray tuchar 64 noattr));
    `(eq (Vptr cb cofs)) (eval_id _ctx); `(eq (Vptr kb kofs)) (eval_id _key);
    `(eq (Vint (Int.repr l))) (eval_id _len);
+   `(eq ctxkey) (eval_var _ctx_key (Tarray tuchar 64 noattr));
    `(eq KV) (eval_var sha._K256 (tarray tuint 64)))
    SEP  (`(K_vector KV);
    `(sha256state_ ipadSHAabs (Vptr cb (Int.add cofs (Int.repr 108))));
    `(data_block Tsh
        (HMAC_SHA256.mkArgZ (map Byte.repr (HMAC_SHA256.mkKey key)) HMAC_SHA256.Opad)
        (Vptr pb pofs));
-   `(field_at Tsh t_struct_hmac_ctx_st [_key_length]
-       (if zlt 64 (Zlength key)
-        then Vint (Int.repr 32)
-        else Vint (Int.repr (Zlength key))) (Vptr cb cofs));
-   `(field_at Tsh t_struct_hmac_ctx_st [_key]
-       (map Vint (map Int.repr (HMAC_SHA256.mkKey key))) (Vptr cb cofs));
    `(data_at Tsh (nested_field_type2 t_struct_hmac_ctx_st [_o_ctx]) emptySha
        (Vptr cb
           (Int.add cofs
              (Int.repr (nested_field_offset2 t_struct_hmac_ctx_st [_o_ctx])))));
    `(field_at Tsh t_struct_hmac_ctx_st [_md_ctx] emptySha (Vptr cb cofs));
+   `(data_at Tsh (tarray tuchar 64)
+       (map Vint (map Int.repr (HMAC_SHA256.mkKey key))) (Vptr ckb ckofs));
    `(array_at tuchar Tsh (tuchars (map Int.repr key)) 0 (Zlength key)
        (Vptr kb kofs))))). 
     { (*opad loop*)
@@ -501,22 +453,19 @@ eapply semax_seq. instantiate (1:=PostResetBranch).
                  `(eq (Vptr cb cofs)) (eval_id _ctx);
                  `(eq (Vptr kb kofs)) (eval_id _key);
                  `(eq (Vint (Int.repr l))) (eval_id _len);
+                 `(eq ctxkey) (eval_var _ctx_key (Tarray tuchar 64 noattr));
                  `(eq KV) (eval_var sha._K256 (tarray tuint 64)))
    SEP  (`(K_vector KV);
    `(sha256state_ ipadSHAabs (Vptr cb (Int.add cofs (Int.repr 108))));
    `(array_at tuchar Tsh OPADcont 0 i (Vptr pb pofs));
    `(array_at tuchar Tsh IPADcont i 64 (Vptr pb pofs));
-   `(field_at Tsh t_struct_hmac_ctx_st [_key_length]
-       (if zlt 64 (Zlength key)
-        then Vint (Int.repr 32)
-        else Vint (Int.repr (Zlength key))) (Vptr cb cofs));
-   `(field_at Tsh t_struct_hmac_ctx_st [_key]
-       (map Vint (map Int.repr (HMAC_SHA256.mkKey key))) (Vptr cb cofs));
    `(data_at Tsh (nested_field_type2 t_struct_hmac_ctx_st [_o_ctx]) emptySha
        (Vptr cb
           (Int.add cofs
              (Int.repr (nested_field_offset2 t_struct_hmac_ctx_st [_o_ctx])))));
    `(field_at Tsh t_struct_hmac_ctx_st [_md_ctx] emptySha (Vptr cb cofs));
+         `(data_at Tsh (tarray tuchar 64)
+              (map Vint (map Int.repr (HMAC_SHA256.mkKey key))) (Vptr ckb ckofs));
    `(array_at tuchar Tsh (tuchars (map Int.repr key)) 0 (Zlength key)
        (Vptr kb kofs))))).
       { (*precondition implies "invariant"*)
@@ -543,10 +492,7 @@ eapply semax_seq. instantiate (1:=PostResetBranch).
             rewrite ZLO. assumption. rewrite Hn. unfold HMAC_SHA256.mkArgZ in Hn; rewrite Hn. trivial.
       }
       { (*unfold_data_at 1%nat. normalize.*)
-        rewrite (field_at_data_at Tsh t_struct_hmac_ctx_st [_key]); try reflexivity.
-        normalize. rename H into I. 
-        rewrite at_offset'_eq.
-        2: simpl; rewrite Int.add_zero; reflexivity.
+        rename H into I. 
         eapply semax_pre0; [ apply now_later | ].
         eapply semax_post_flipped'.
         { subst PostResetBranch.
@@ -558,37 +504,11 @@ eapply semax_seq. instantiate (1:=PostResetBranch).
                    (HMAC_SHA256.mkArgZ (map Byte.repr (HMAC_SHA256.mkKey key)) HMAC_SHA256.Opad))) i
               = Vint (Int.zero_ext 8 (Int.xor (Int.repr 92) N))). 
           { clear - HN I isbyte_key. apply xor_pad_result; assumption. }
+          unfold tarray. 
+          erewrite data_at_array_at with (v:= map Vint (map Int.repr (HMAC_SHA256.mkKey key))); try reflexivity.
+              2: omega. 
           eapply NEWsemax_loadstore_array
-          with (P:= nil)
-          (Q:= [`(eq (Vint (Int.repr i))) (eval_id _i);
-            `(eq (Vint (Int.repr 64))) (eval_expr (Econst_int (Int.repr 64) tint));
-            `(eq (Vint (Int.repr 1))) (eval_id _reset);
-            `(eq (Vptr pb pofs)) (eval_var _pad (tarray tuchar 64));
-            `(eq (Vptr cb cofs)) (eval_id _ctx);
-            `(eq (Vptr kb kofs)) (eval_id _key);
-            `(eq (Vint (Int.repr l))) (eval_id _len);
-            `(eq KV) (eval_var sha._K256 (tarray tuint 64))])
-          (R:= [`(K_vector KV);
-     `(sha256state_ ipadSHAabs (Vptr cb (Int.add cofs (Int.repr 108))));
-     `(array_at tuchar Tsh OPADcont 0 i (Vptr pb pofs));
-     `(array_at tuchar Tsh IPADcont i 64 (Vptr pb pofs));
-     `(field_at Tsh t_struct_hmac_ctx_st [_key_length]
-         (if zlt 64 (Zlength key)
-          then Vint (Int.repr 32)
-          else Vint (Int.repr (Zlength key))) (Vptr cb cofs));
-     `(data_at Tsh (nested_field_type2 t_struct_hmac_ctx_st [_key])
-         (map Vint (map Int.repr (HMAC_SHA256.mkKey key)))
-         (offset_val
-            (Int.repr (nested_field_offset2 t_struct_hmac_ctx_st [_key]))
-            (Vptr cb cofs)));
-     `(data_at Tsh (nested_field_type2 t_struct_hmac_ctx_st [_o_ctx])
-         emptySha
-         (Vptr cb
-            (Int.add cofs
-               (Int.repr (nested_field_offset2 t_struct_hmac_ctx_st [_o_ctx])))));
-     `(field_at Tsh t_struct_hmac_ctx_st [_md_ctx] emptySha (Vptr cb cofs));
-     `(array_at tuchar Tsh (tuchars (map Int.repr key)) 0 (Zlength key)
-         (Vptr kb kofs))])
+          with 
           (n:=3%nat)
           (v2:=(ZnthV tuchar (map Vint(map Int.repr (HMAC_SHA256.mkArgZ (map Byte.repr (HMAC_SHA256.mkKey key)) HMAC_SHA256.Opad))) i)).
           simpl; try reflexivity.
@@ -596,41 +516,31 @@ eapply semax_seq. instantiate (1:=PostResetBranch).
           simpl; try reflexivity.
           simpl; try reflexivity.
           simpl; try reflexivity.
-          Focus 2. simpl. unfold value, nested_field_type2, t_struct_hmac_ctx_st; simpl.
-            reflexivity.
-          2: trivial.
-          instantiate (1:=i). unfold nested_field_offset2, _struct_SHA256state_st; simpl.
-          intros rho. normalize.
-           apply andp_right. apply andp_right; rel_expr.
-           rewrite Hres.
-           erewrite (data_at_type_changable Tsh _ (tarray tuchar 64)); try reflexivity.
-           unfold tarray. 
-           erewrite data_at_array_at; try reflexivity.
-           erewrite (split3_array_at' i _ _ _ 0 64); try reflexivity. 2: trivial. 2: omega.
-           { rel_expr. 
-              instantiate (1:=cofs). instantiate (1:=cb). admit. (* rel_expr.*)
-             unfold nested_field_offset2, _struct_SHA256state_st; simpl.
-              instantiate (2:=Tsh). unfold add_ptr_int. simpl.
-              instantiate (1:=(ZnthV tuchar (map Vint (map Int.repr (HMAC_SHA256.mkKey key))) i)).
-              cancel.
-             unfold ZnthV in *. if_tac. omega. simpl; rewrite HN. discriminate.
-             simpl; intros.
+          { instantiate (1:=i). instantiate (1:=Vptr pb pofs).
+            entailer. normalize. 
+            apply andp_right. apply andp_right; rel_expr. 
+            rewrite Hres. 
+            erewrite (split3_array_at' i _ _ _ 0 64); try reflexivity. 2: trivial.
+            { rel_expr. 
+              unfold ZnthV in *. if_tac. omega. simpl; rewrite HN. discriminate.
+              simpl; intros.
                 unfold ZnthV in *. if_tac. omega. simpl; rewrite HN. reflexivity.
-             reflexivity.
-           }
-           { unfold HMAC_SHA256.mkArgZ. simpl. apply ZnthV_map_Vint_is_int_I8.
-             unfold HMAC_SHA256.mkArgZ in ZLO. rewrite Zlength_correct, map_length in ZLO. 
-             rewrite Zlength_correct, ZLO. omega.
-           }
-           red; omega. 
-        }
+              reflexivity. 
+            }
+          }
+          simpl. reflexivity.
+          trivial.
+          { unfold HMAC_SHA256.mkArgZ. simpl. apply ZnthV_map_Vint_is_int_I8.
+            unfold HMAC_SHA256.mkArgZ in ZLO. rewrite Zlength_correct, map_length in ZLO. 
+            rewrite Zlength_correct, ZLO. omega.
+          }
+          red; omega.   
+          }
         { entailer. cancel.
           rewrite (split_array_at (i+1) tuchar Tsh _ i 64); try omega. cancel.
-          unfold_data_at 1%nat. cancel.
-          rewrite (field_at_data_at Tsh t_struct_hmac_ctx_st [_key]); try reflexivity.
-          rewrite at_offset'_eq.
-            2: simpl; rewrite Int.add_zero; reflexivity. unfold offset_val.
-          unfold_data_at 1%nat. entailer. cancel.
+          unfold tarray. erewrite data_at_array_at; try reflexivity.
+              2: omega.
+          cancel. 
           apply sepcon_derives.
             rewrite (split_array_at i tuchar Tsh _ 0 (i+1)); try omega.
             cancel.
@@ -640,7 +550,7 @@ eapply semax_seq. instantiate (1:=PostResetBranch).
             destruct (zlt i 0). omega. simpl. rewrite upd_eq.
             destruct (nth_mapVintZ i 
              (HMAC_SHA256.mkArgZ (map Byte.repr (HMAC_SHA256.mkKey key)) HMAC_SHA256.Opad)) as [n Hn].
-              rewrite ZLO; assumption.
+             rewrite ZLO; assumption.
             rewrite Hn. unfold HMAC_SHA256.mkArgZ in Hn; rewrite Hn. trivial.
           apply array_lemmas.array_at_ext'.
             unfold cVint, ZnthV; simpl; intros. rewrite upd_neq; trivial. omega.
@@ -654,7 +564,7 @@ eapply semax_seq. instantiate (1:=PostResetBranch).
     rewrite at_offset'_eq.
     2: simpl; rewrite Int.add_zero; reflexivity.*)
     eapply semax_seq'.
-    frame_SEP 5.
+    frame_SEP 3.
     forward_call (Vptr cb (Int.add cofs (Int.repr 216))).
     { assert (FR: Frame = nil).
         subst Frame. reflexivity.
@@ -673,13 +583,9 @@ eapply semax_seq. instantiate (1:=PostResetBranch).
     forward_call WITNESS.
     { assert (FR: Frame = [
          `(sha256state_ ipadSHAabs (Vptr cb (Int.add cofs (Int.repr 108))));
-         `(field_at Tsh t_struct_hmac_ctx_st [_key_length]
-              (if zlt 64 (Zlength key)
-               then Vint (Int.repr 32)
-               else Vint (Int.repr (Zlength key))) (Vptr cb cofs));
-         `(field_at Tsh t_struct_hmac_ctx_st [_key]
-              (map Vint (map Int.repr (HMAC_SHA256.mkKey key))) (Vptr cb cofs));
          `(field_at Tsh t_struct_hmac_ctx_st [_md_ctx] emptySha (Vptr cb cofs));
+         `(data_at Tsh (tarray tuchar 64)
+            (map Vint (map Int.repr (HMAC_SHA256.mkKey key))) (Vptr ckb ckofs));
          `(array_at tuchar Tsh (tuchars (map Int.repr key)) 0 (Zlength key)
               (Vptr kb kofs))]). 
         subst Frame. reflexivity.
@@ -687,44 +593,45 @@ eapply semax_seq. instantiate (1:=PostResetBranch).
       subst WITNESS. entailer. cancel.
     }
     after_call. simpl. intros rho. subst WITNESS PostResetBranch.
-        rewrite firstn_precise. entailer.
-        rename x into opadSHAabs.
-        unfold sha256state_; normalize. rename r into iUpd. rename x into oUpd.
-        apply exp_right with (x:=ipadSHAabs). entailer.
-        apply exp_right with (x:=iUpd). entailer.
-        apply exp_right with (x:=opadSHAabs). entailer.
-        apply exp_right with (x:=oUpd). entailer.
-        unfold data_block, initPostResetConditional. simpl.
-        rewrite ZLO. entailer. cancel.
-        unfold_data_at 3%nat. cancel.
-    rewrite (field_at_data_at Tsh t_struct_hmac_ctx_st [_i_ctx]); try reflexivity.
-    entailer.
-    rewrite at_offset'_eq.
-    2: simpl; rewrite Int.add_zero; reflexivity. unfold offset_val; simpl.
+    rewrite firstn_precise.
+    { entailer.
+      rename x into opadSHAabs.
+      unfold sha256state_; normalize. rename r into iUpd. rename x into oUpd.
+      apply exp_right with (x:=ipadSHAabs). entailer.
+      apply exp_right with (x:=iUpd). entailer.
+      apply exp_right with (x:=opadSHAabs). entailer.
+      apply exp_right with (x:=oUpd). entailer.
+      unfold data_block, initPostResetConditional. simpl.
+      rewrite ZLO. entailer. apply exp_right with (x:=l). entailer. cancel.
+      unfold_data_at 3%nat. cancel.
+      rewrite (field_at_data_at Tsh t_struct_hmac_ctx_st [_i_ctx]); try reflexivity.
+      entailer.
+      rewrite at_offset'_eq.
+      2: simpl; rewrite Int.add_zero; reflexivity. unfold offset_val; simpl.
 
-    rewrite (field_at_data_at Tsh t_struct_hmac_ctx_st [_o_ctx]); try reflexivity.
-    entailer.
-    rewrite at_offset'_eq.
-    2: simpl; rewrite Int.add_zero; reflexivity. unfold offset_val; simpl.
+      rewrite (field_at_data_at Tsh t_struct_hmac_ctx_st [_o_ctx]); try reflexivity.
+      entailer.
+      rewrite at_offset'_eq.
+      2: simpl; rewrite Int.add_zero; reflexivity. unfold offset_val; simpl.
 
-    cancel.
+      cancel. 
+    }
 
-      unfold HMAC_SHA256.mkArgZ, HMAC_SHA256.mkArg. repeat rewrite map_length.
-      unfold HMAC_SHA256.sixtyfour. rewrite combine_length, map_length, length_Nlist, mkKey_length.
-      unfold SHA256.BlockSize; simpl. trivial.
+    unfold HMAC_SHA256.mkArgZ, HMAC_SHA256.mkArg. repeat rewrite map_length.
+    unfold HMAC_SHA256.sixtyfour. rewrite combine_length, map_length, length_Nlist, mkKey_length.
+    unfold SHA256.BlockSize; simpl. trivial.
   }
   { (*ELSE*) 
     forward. unfold overridePost. simpl. intros rho. apply andp_right. apply prop_right. trivial.
     subst. unfold initPostKeyNullConditional; simpl. entailer.
     rewrite <- H1 in *; simpl in *. unfold typed_false in H0. simpl in H0.
-        inversion H0; clear H0. apply negb_false_iff in H6.
-        apply eq_sym in H6; apply binop_lemmas.int_eq_true in H6.
+        inversion H0; clear H0. apply negb_false_iff in H5.
+        apply eq_sym in H5; apply binop_lemmas.int_eq_true in H5.
     destruct R; subst. simpl.
       remember (eval_id _key rho) as k. destruct k; entailer. 
       remember (Int.eq i Int.zero) as d. destruct d. 2: entailer.
       unfold hmacstate_PreInitNull, hmac_relate_PreInitNull; simpl.
       destruct h1; entailer.
-       destruct H10 as [ii [KLi [KLunsig [SF [ISHA OSHA]]]]].
        apply exp_right with (x:= iSha). 
        apply exp_right with (x:= (iCtx r)).
        apply exp_right with (x:= oSha).
@@ -733,8 +640,8 @@ eapply semax_seq. instantiate (1:=PostResetBranch).
        unfold hmacstate_PreInitNull, hmac_relate_PreInitNull; simpl.
        apply sepcon_derives. unfold tarray. rewrite data_at__array_at_. cancel. omega. reflexivity.        
        apply exp_right with (x:= r). apply exp_right with (x:=v).
-       entailer. apply prop_right. exists ii; eauto.
-     simpl. apply Int.one_not_zero in H6. contradiction.
+       entailer. 
+     simpl. apply Int.one_not_zero in H5. contradiction.
    } 
 }
 { (*Continuation after if (reset*)
@@ -761,8 +668,8 @@ apply semax_extensionality_Delta with (Delta). apply expr_lemmas.tycontext_sub_r
      unfold hmac_relate_PreInitNull in Hs. 
      clear INNER InnerRelate OUTER OuterRelate iSA iS oSA oS.
      destruct h1.
-     destruct Hs as [XX [IREL [OREL [ILEN [OLEN [KK [ii [KLii [KL [HH1 [HH2 HH3]]]]]]]]]]].
-     subst key0. destruct s as [mdS [iS [oS [kl K]]]]. simpl in *. subst kl K.
+     destruct Hs as [IREL [OREL [ILEN [OLEN [ISHA OSHA]]]]].
+     destruct s as [mdS [iS oS]]. simpl in *.
      unfold_data_at 1%nat.
      (* eapply semax_seq'.
      frame_SEP 3 4.*)
@@ -779,10 +686,8 @@ apply semax_extensionality_Delta with (Delta). apply expr_lemmas.tycontext_sub_r
              mkTrep t_struct_SHA256state_st iS) as  WITNESS.
      forward_call WITNESS.
      { assert (FR: Frame = [
-          `(field_at Tsh t_struct_hmac_ctx_st [_key_length] (Vint ii) (Vptr cb cofs)); 
-          `(field_at Tsh t_struct_hmac_ctx_st [_key]
-               (map Vint (map Int.repr (HMAC_SHA256.mkKey key))) (Vptr cb cofs));
           `(field_at Tsh t_struct_hmac_ctx_st [_o_ctx] oS (Vptr cb cofs));
+          `(data_at_ Tsh (tarray tuchar 64) ctxkey);
           `(array_at_ tuchar Tsh 0 64 pad); `(K_vector KV)]).
           subst Frame. reflexivity.
        rewrite FR. clear FR Frame. 
@@ -798,46 +703,41 @@ apply semax_extensionality_Delta with (Delta). apply expr_lemmas.tycontext_sub_r
      after_call. subst WITNESS. normalize. subst retval0. simpl. 
 
      forward. (*return*)
-     unfold hmacInit. 
+     unfold hmacInit. (**)
      remember (Int.unsigned (Int.repr (if zlt 64 (Zlength key) then 32 else Zlength key)))as KL.
-     apply exp_right with (x:=HMACabs iSha iSha oSha KL key).   
+     apply exp_right with (x:=HMACabs iSha iSha oSha).   
      entailer.
      apply andp_right. 
-       apply prop_right. exists iSha, oSha.
+       apply prop_right. exists iSha, oSha. auto. (*
        rewrite Int.unsigned_repr. auto.
        rewrite int_max_signed_eq  in KL2. rewrite int_max_unsigned_eq.
-       destruct (zlt 64 (Zlength key)); omega.     
+       destruct (zlt 64 (Zlength key)); omega.     *)
      simpl_stackframe_of. unfold tarray. 
      rewrite <- data_at__array_at_ with (a:=noattr).
      2: omega. 2: reflexivity.
      cancel.
      unfold hmacstate_, hmac_relate.
-      remember (if zlt 64 (Zlength key) then Vint (Int.repr 32)
-            else Vint (Int.repr (Zlength key))) as kl.
+(*      remember (if zlt 64 (Zlength key) then Vint (Int.repr 32)
+            else Vint (Int.repr (Zlength key))) as kl.*)
       normalize.
-      apply exp_right with
-        (x:=(iS, (iS, (oS, (kl, map Vint (map Int.repr (HMAC_SHA256.mkKey key))))))).
-      simpl.
-      apply andp_right. apply prop_right. repeat split; trivial.
-      destruct (zlt 64 (Zlength key)); simpl in *.
-         exists (Int.repr 32); eauto.
-         rewrite Heqkl, HH1. exists (Int.repr (Int.unsigned ii)).
-         rewrite Int.repr_unsigned; eauto.
+      apply exp_right with (x:=(iS, (iS, oS))).
+      simpl. entailer.
+(*      apply andp_right. apply prop_right.
+      destruct (zlt 64 (Zlength key)); simpl in *. trivial.
+          rewrite Int.unsigned_repr. trivial. 
+           rewrite int_max_unsigned_eq. rewrite int_max_signed_eq in KL2. omega.*)
 
       unfold_data_at 3%nat. cancel.
       rewrite (field_at_data_at Tsh t_struct_hmac_ctx_st [_i_ctx]); try reflexivity.
       rewrite (field_at_data_at Tsh t_struct_hmac_ctx_st [_md_ctx]); try reflexivity.
-      entailer. cancel.
-      destruct (zlt 64 (Zlength key)); simpl in *;
-        rewrite HH1, Int.repr_unsigned; simpl in *.
-        cancel.
-        cancel.
+      entailer. 
   }
 
   { (*k is Vptr, key!=NULL*)
     destruct R; subst r; simpl. 
     apply semax_pre with (P':=FF); try entailer; try apply semax_ff.
-    normalize. 
+    normalize. intros ll. normalize. subst l; rename ll into l.
+    rename H into isbyteKey. rename H0 into KL. 
     unfold postResetHMS. simpl. unfold_data_at 1%nat.
     (* eapply semax_seq'.
     frame_SEP 3 4.*)
@@ -851,19 +751,15 @@ apply semax_extensionality_Delta with (Delta). apply expr_lemmas.tycontext_sub_r
       LOCAL  (`(eq pad) (eval_var _pad (tarray tuchar 64));
        `(eq (Vptr cb cofs)) (eval_id _ctx); `(eq (Vptr kb kofs)) (eval_id _key);
        `(eq (Vint (Int.repr l))) (eval_id _len);
+       `(eq ctxkey) (eval_var _ctx_key (tarray tuchar 64));
        `(eq KV) (eval_var sha._K256 (tarray tuint 64)))
-      SEP  (`(field_at Tsh t_struct_hmac_ctx_st [_key_length]
-            (if zlt 64 (Zlength key)
-            then Vint (Int.repr 32)
-            else Vint (Int.repr (Zlength key))) (Vptr cb cofs));
+      SEP  (
           `(field_at Tsh t_struct_hmac_ctx_st [_o_ctx] oS (Vptr cb cofs));
-          `(field_at Tsh t_struct_hmac_ctx_st [_key]
-              (map Vint (map Int.repr (HMAC_SHA256.mkKey key))) (Vptr cb cofs));
           `(field_at Tsh t_struct_hmac_ctx_st [_i_ctx] iS (Vptr cb cofs));
           `(data_at_ Tsh (tarray tuchar 64) pad);
           `(array_at tuchar Tsh (tuchars (map Int.repr key)) 0 (Zlength key)
               (Vptr kb kofs));
-          `(K_vector KV);
+          `(data_at_ Tsh (tarray tuchar 64) ctxkey); `(K_vector KV);
           `(memory_block Tsh (Int.repr (sizeof (nested_field_type2 t_struct_hmac_ctx_st [_md_ctx])))
              (offset_val
                 (Int.repr (nested_field_offset2 t_struct_hmac_ctx_st [_md_ctx]))
@@ -888,13 +784,8 @@ apply semax_extensionality_Delta with (Delta). apply expr_lemmas.tycontext_sub_r
              mkTrep t_struct_SHA256state_st iS) as  WITNESS.
     forward_call WITNESS.
     { assert (FR: Frame = [
-         `(field_at Tsh t_struct_hmac_ctx_st [_key_length]
-            (if zlt 64 (Zlength key)
-             then Vint (Int.repr 32)
-             else Vint (Int.repr (Zlength key))) (Vptr cb cofs));
          `(field_at Tsh t_struct_hmac_ctx_st [_o_ctx] oS (Vptr cb cofs));
-         `(field_at Tsh t_struct_hmac_ctx_st [_key]
-            (map Vint (map Int.repr (HMAC_SHA256.mkKey key))) (Vptr cb cofs));
+         `(data_at_ Tsh (tarray tuchar 64) ctxkey);
          `(data_at_ Tsh (tarray tuchar 64) pad);
          `(array_at tuchar Tsh (tuchars (map Int.repr key)) 0 (Zlength key)
             (Vptr kb kofs)); `(K_vector KV)]).
@@ -905,33 +796,19 @@ apply semax_extensionality_Delta with (Delta). apply expr_lemmas.tycontext_sub_r
     after_call. subst WITNESS. normalize.  subst retval0. simpl. 
 
     forward. (*return*)
-    remember (Int.unsigned (Int.repr (if zlt 64 (Zlength key) then 32 else Zlength key)))as KL.
-    apply exp_right with (x:=HMACabs iSA iSA oSA KL key). 
+    apply exp_right with (x:=HMACabs iSA iSA oSA). 
     entailer.
     apply andp_right. 
-      apply prop_right. unfold hmacInit. exists iSA, oSA.
-      rewrite Int.unsigned_repr. auto.
-      rewrite int_max_signed_eq  in KL2. rewrite int_max_unsigned_eq.
-      destruct (zlt 64 (Zlength key)); omega.    
+      apply prop_right. unfold hmacInit. exists iSA, oSA. auto.
     unfold data_block. simpl_stackframe_of. entailer. cancel.
     unfold hmacstate_, hmac_relate.
-    remember (if zlt 64 (Zlength key) then Vint (Int.repr 32)
-              else Vint (Int.repr (Zlength key))) as kl.
-    normalize.
-    apply exp_right with
-      (x:=(iS, (iS, (oS, (kl, map Vint (map Int.repr (HMAC_SHA256.mkKey key))))))).
+    apply exp_right with (x:=(iS, (iS, oS))).
     simpl. entailer.
     apply andp_right. apply prop_right.
       split. rewrite (updAbs_len _ _ _ INNER), Zlength_mkArgZ,
            map_length, mkKey_length; reflexivity.
-      split. rewrite (updAbs_len _ _ _ OUTER), Zlength_mkArgZ,
+      rewrite (updAbs_len _ _ _ OUTER), Zlength_mkArgZ,
            map_length, mkKey_length; reflexivity.
-      exists (Int.repr (if zlt 64 (Zlength key) then 32 else Zlength key)).
-      rewrite Int.unsigned_repr. 
-      split. destruct (zlt 64 (Zlength key)); trivial.
-      split; trivial.
-      rewrite int_max_signed_eq  in KL2. rewrite int_max_unsigned_eq.
-      destruct (zlt 64 (Zlength key)); omega.
 
     unfold_data_at 3%nat. cancel.
     rewrite (field_at_data_at Tsh t_struct_hmac_ctx_st [_i_ctx]); try reflexivity.
