sha/verif_hmacADT_update.v
@@ -1,0 +1,84 @@
+Require Import floyd.proofauto.
+Import ListNotations.
+Require sha.sha.
+Require sha.SHA256.
+Local Open Scope logic.
+
+Require Import sha.spec_sha.
+Require Import sha_lemmas.
+Require Import sha.HMAC_functional_prog.
+
+Require Import sha.hmac_NK.
+Require Import sha.spec_hmacADT.
+
+Lemma body_hmac_update: semax_body HmacVarSpecs HmacFunSpecs 
+       f_HMAC_Update HMAC_Update_spec.
+Proof.
+start_function.
+name ctx' _ctx.
+name data' _data.
+name len' _len.
+unfold hmacstate_. normalize. intros ST. normalize.
+destruct H as [DL1 [DL2 DL3]].
+destruct h1; simpl in *.
+destruct H0 as [reprMD [reprI [reprO [iShaLen oShaLen]]]].
+(*rewrite KL in *.*)
+erewrite (field_except_at_lemma _ _ _md_ctx nil); try reflexivity.
+simpl. 
+
+(*By rewriting with field_at_data_at here instead of inside the forward_call,
+  we remember facts SCc and ACc which are necessary for performing the
+  "inverse" conversion at the end of this proof*)  
+rewrite field_at_data_at; try reflexivity. simpl. normalize. 
+rename H into SCc. rename H0 into ACc.
+
+eapply semax_seq'. 
+frame_SEP 0 2 3.
+remember (ctx, data, c, d, Tsh, len, KV) as WITNESS.
+forward_call WITNESS.
+  { assert (FR: Frame =nil).
+       subst Frame. reflexivity.
+    rewrite FR. clear FR Frame. 
+    subst WITNESS. entailer.
+    cancel. 
+    unfold sha256state_. apply exp_right with (x:= mdCtx ST). entailer.
+    (*rewrite field_at_data_at; try reflexivity. simpl. entailer.*)
+  }
+after_call. subst WITNESS. normalize. simpl. (* normalize.*)
+
+assert (FF: firstn (Z.to_nat len) data = data). 
+    rewrite DL1 in *. 
+    apply firstn_same. rewrite Zlength_correct, Nat2Z.id. omega.
+rewrite FF in *. 
+
+(**** Again, distribute EX over lift*)
+apply semax_pre with (P' :=EX  x : s256abs,
+  (PROP  ()
+   LOCAL  (tc_environ Delta; `(eq c) (eval_id _ctx); `(eq d) (eval_id _data);
+   `(eq (Vint (Int.repr len))) (eval_id _len);
+   `(eq KV) (eval_var sha._K256 (tarray tuint 64)))
+   SEP 
+   (`(fun a : environ =>
+      (PROP  (update_abs data ctx x)
+       LOCAL ()
+       SEP  (`(K_vector KV); `(sha256state_ x c); `(data_block Tsh data d)))
+        a) globals_only;
+   `(field_except_at Tsh t_struct_hmac_ctx_st _md_ctx [] (snd ST) c)))).
+  entailer. rename x into s. apply exp_right with (x:=s). entailer.
+apply extract_exists_pre. intros s. normalize. simpl. normalize.
+(********************************************************)
+rename H into HmacUpdate.
+
+(*WHY IS THIS NEEDED?*) unfold MORE_COMMANDS, abbreviate.
+forward.
+apply exp_right with (x:= HMACabs s iSha oSha). entailer.
+apply andp_right. apply prop_right. exists s; eauto.
+cancel. 
+unfold hmacstate_, sha256state_, hmac_relate. normalize.
+apply exp_right with (x:=(r, (iCtx ST, oCtx ST))). 
+simpl. entailer.
+(*apply andp_right. apply prop_right. exists l; eauto.*)
+erewrite (field_except_at_lemma Tsh t_struct_hmac_ctx_st _md_ctx nil); try reflexivity.
+destruct ST as [ST1 [ST2 ST3]]. simpl in *. cancel.
+rewrite field_at_data_at; try reflexivity. simpl. normalize. 
+Qed.
